Update on the lemmas

ProvingItemIndex.fst
@@ -9,101 +9,78 @@ open FStar.List.Tot.Base
 type english_letters =
   | A
   | B
-  // | C 
-  // | D
-  // | E
-  // | F 
-  // | G
-  // | H
-  // | I 
-  // | J
-  // | K
-  // | L 
-  // | M 
-  // | N 
-  // | O 
-  // | P 
-  // | Q 
-  // | R 
-  // | S 
-  // | T 
-  // | U 
-  // | V 
-  // | W 
-  // | X 
-  // | Y 
-  // | Z
 
 val alphabet : (l:list english_letters{(forall (x:english_letters). mem x l = true) /\ l <> []})
-let alphabet = [A;B]//;C;D;E;F;G;H;I;J;K;M;N;O;P;Q;R;S;T;U;V;W;X;Y;Z]
+let alphabet = [A;B]
   
 val text : (l:list english_letters{l <> []})
 let text = [A;A;A;A;B;A;A;B;A;B;A;A;A;B;A;B;B]
 
+let rec l1_length_less_than_l2_length (l1:list english_letters) (l2:list english_letters)
+  : bool
+  = if length l1 > 0 && length l2 > 0 
+    then l1_length_less_than_l2_length (tail l1) (tail l2)
+    else (
+      if length l1 = 0 
+      then true
+      else false
+    )
+
+let rec l1_less_true (l1:list english_letters) (l2:list english_letters)
+  : Lemma (requires l1_length_less_than_l2_length l1 l2 = true)
+          (ensures length l1 <= length l2)
+  = if length l1 > 0 && length l2 > 0 
+    then l1_less_true (tail l1) (tail l2)
+    else ()
+
+let rec l1_less_false (l1:list english_letters) (l2:list english_letters)
+  : Lemma (requires l1_length_less_than_l2_length l1 l2 = false)
+          (ensures length l1 > length l2)
+  = if length l1 > 0 && length l2 > 0 
+    then l1_less_false (tail l1) (tail l2)
+    else ()
+
+let candidate : list english_letters 
+  = [B;A;B;A;A;A;B;A;B]
+
 val pattern : (l:list english_letters{length l <= length text})
-let pattern = [A;B;B]
+let pattern = if l1_length_less_than_l2_length candidate text = true
+              then (
+                l1_less_true candidate text;
+                candidate
+              )
+              else []
 
-val alphabet_length : (i:nat{i > 0})
-let alphabet_length = length alphabet
-
-let rec create_bc (i:nat) : Tot (list int) (decreases i) 
-  =match i with
-      | 0 -> []
-      | _ -> (-1) :: (create_bc (i-1))
-
-let rec length_create_bc_is_positive (i:nat)
-  : Lemma (ensures length (create_bc i) >= 0)
-  = match i with
-    | 0 -> ()
-    | _ -> length_create_bc_is_positive (i - 1)
-
-let rec length_create_bc_is_i (i:nat) :
-   Lemma (ensures (length (create_bc i) = i)) =
-   match i with 
-     | 0 -> ()
-     | _ -> length_create_bc_is_i (i - 1)
-
-let rec index_n_bc_is_minusone (i:nat) :
-  Lemma (ensures 
-        (let l = (create_bc i) in 
-         forall (n:nat). n < length l ==> index l n = -1))
-  = match i with
-    | 0 -> ()
-    | _ -> index_n_bc_is_minusone (i - 1)
-
-let bc : list int = create_bc alphabet_length
-
-let bc_length_is_positive = length_create_bc_is_positive alphabet_length
-let bc_length_is_alphabet = length_create_bc_is_i alphabet_length
-let bc_nth_element_is_minusone = index_n_bc_is_minusone alphabet_length
-
-//indices
-val item_index (#a:eqtype) (item:a) (l:list a) (i:nat) : list nat
-let rec item_index item l i
+let rec item_indices (#a:eqtype) (item:a) (l:list a) (i:nat) 
+  : list nat
   = match l with 
     | [] -> []
     | hd :: tl -> if hd = item
-                  then i :: item_index item tl (i + 1)
-                  else item_index item tl (i + 1)
+                  then i :: item_indices item tl (i + 1)
+                  else item_indices item tl (i + 1)
 
 let rec item_list_has_correct_length (#a:eqtype) (l:list a) (i:nat)
-  : Lemma (ensures forall (item:a). length (item_index item l i) = count item l)
+  : Lemma (ensures forall (item:a). length (item_indices item l i) = count item l)
   = match l with 
     | [] -> ()
     | hd :: tl -> item_list_has_correct_length tl (i + 1)
 
 let rec item_indices_is_in_interval (#a:eqtype) (item:a) (l:list a) (i:nat) (x:nat)
-  : Lemma (ensures mem x (item_index item l i) ==> i <= x && x < i + length l)
+  : Lemma (ensures mem x (item_indices item l i) ==> i <= x && x < i + length l)
   = match l with 
     | [] -> () 
     | hd :: tl -> item_indices_is_in_interval item tl (i + 1) x 
 
-let item_indices_is_in_interval_forall (#a:eqtype) (item:a) (l:list a) (i:nat)
-  : Lemma (ensures forall (x:nat). mem x (item_index item l i) ==> i <= x && x < i + length l)
+let item_indices_is_in_interval_forall (#a:eqtype) (l:list a) (i:nat) (item:a)
+  : Lemma (ensures forall (x:nat). mem x (item_indices item l i) ==> i <= x && x < i + length l)
   = forall_intro (item_indices_is_in_interval item l i)
 
+let item_indices_is_in_interval_forall_item (#a:eqtype) (l:list a) (i:nat)
+  : Lemma (ensures forall (item:a) (x:nat). mem x (item_indices item l i) ==> i <= x && x < i + length l)
+  = forall_intro (item_indices_is_in_interval_forall l i)
+
 let rec item_indices_one_and_item_indices_zero (#a:eqtype) (item:a) (l:list a) (x:nat{x > 0}) (i:nat{i > 0})
-  : Lemma (ensures mem x (item_index item l i) = mem (x - 1) (item_index item l (i - 1)))
+  : Lemma (ensures mem x (item_indices item l i) = mem (x - 1) (item_indices item l (i - 1)))
   = match l with 
     | [] -> ()
     | hd :: tl -> match x with 
@@ -136,14 +113,14 @@ let rec item_indices_one_and_item_indices_zero (#a:eqtype) (item:a) (l:list a) (
                             )
                           )
                           else (
-                            assert(mem x (item_index item l i) = mem x (item_index item tl (i + 1)));
-                            assert(mem (x - 1) (item_index item l (i - 1)) = mem (x - 1) (item_index item tl i));
+                            assert(mem x (item_indices item l i) = mem x (item_indices item tl (i + 1)));
+                            assert(mem (x - 1) (item_indices item l (i - 1)) = mem (x - 1) (item_indices item tl i));
                             item_indices_one_and_item_indices_zero item tl x (i + 1)
                           )
                          )
 
 let rec index_increases_with_one_when_element_is_added (#a:eqtype) (item:a) (l:list a) (i:nat{i > 0}) (el:a)
-  : Lemma (ensures mem (i - 1) (item_index item l 0) = false ==> mem i (item_index item (el :: l) 0) = false)
+  : Lemma (ensures mem (i - 1) (item_indices item l 0) = false ==> mem i (item_indices item (el :: l) 0) = false)
   = match l with 
     | [] -> ()
     | hd :: tl -> match i with 
@@ -154,7 +131,7 @@ let rec index_increases_with_one_when_element_is_added (#a:eqtype) (item:a) (l:l
                          index_increases_with_one_when_element_is_added item tl (i - 1) hd
 
 let rec index_increases_with_one_when_element_is_added_for_true (#a:eqtype) (item:a) (l:list a) (i:nat{i > 0}) (el:a)
-  : Lemma (ensures mem (i - 1) (item_index item l 0) = true ==> mem i (item_index item (el :: l) 0) = true)
+  : Lemma (ensures mem (i - 1) (item_indices item l 0) = true ==> mem i (item_indices item (el :: l) 0) = true)
   = match l with 
     | [] -> ()
     | hd :: tl -> match i with 
@@ -165,7 +142,7 @@ let rec index_increases_with_one_when_element_is_added_for_true (#a:eqtype) (ite
                          index_increases_with_one_when_element_is_added_for_true item tl (i - 1) hd
 
 let rec index_increases_with_one_when_first_is_item (#a:eqtype) (item:a) (l:list a) (i:nat{i > 0})
-  : Lemma (ensures mem (i - 1) (item_index item l 0) = false ==> mem i (0 :: item_index item l 1) = false)
+  : Lemma (ensures mem (i - 1) (item_indices item l 0) = false ==> mem i (0 :: item_indices item l 1) = false)
   = match l with 
     | [] -> ()
     | hd :: tl -> match i with 
@@ -176,7 +153,7 @@ let rec index_increases_with_one_when_first_is_item (#a:eqtype) (item:a) (l:list
                          index_increases_with_one_when_first_is_item item tl (i - 1)
 
 let rec index_increases_with_one_when_first_is_item_for_true (#a:eqtype) (item:a) (l:list a) (i:nat{i > 0})
-  : Lemma (ensures mem (i - 1) (item_index item l 0) = true ==> mem i (0 :: item_index item l 1) = true)
+  : Lemma (ensures mem (i - 1) (item_indices item l 0) = true ==> mem i (0 :: item_indices item l 1) = true)
   = match l with 
     | [] -> ()
     | hd :: tl -> match i with 
@@ -187,7 +164,7 @@ let rec index_increases_with_one_when_first_is_item_for_true (#a:eqtype) (item:a
                          index_increases_with_one_when_first_is_item_for_true item tl (i - 1)
 
 let rec index_is_not_item_is_not_mem_base (#a:eqtype) (l:list a) (item:a) (i:nat{i < length l})
-  : Lemma (ensures index l i <> item ==> mem i (item_index item l 0) = false)
+  : Lemma (ensures index l i <> item ==> mem i (item_indices item l 0) = false)
   = match l with
     | [] -> ()
     | hd :: tl -> match i with 
@@ -200,11 +177,11 @@ let rec index_is_not_item_is_not_mem_base (#a:eqtype) (l:list a) (item:a) (i:nat
                          index_is_not_item_is_not_mem_base tl item (i - 1)
 
 let index_is_not_item_is_not_mem (#a:eqtype) (l:list a) 
-  : Lemma (ensures forall (item:a) (i:nat{i < length l}). index l i <> item ==> mem i (item_index item l 0) = false)
+  : Lemma (ensures forall (item:a) (i:nat{i < length l}). index l i <> item ==> mem i (item_indices item l 0) = false)
   = forall_intro_2 (index_is_not_item_is_not_mem_base l)
 
 let rec index_is_item_is_mem_base (#a:eqtype) (l:list a) (item:a) (i:nat{i < length l})
-  : Lemma (ensures index l i = item ==> mem i (item_index item l 0) = true)
+  : Lemma (ensures index l i = item ==> mem i (item_indices item l 0) = true)
   = match l with
     | [] -> ()
     | hd :: tl -> match i with 
@@ -218,11 +195,11 @@ let rec index_is_item_is_mem_base (#a:eqtype) (l:list a) (item:a) (i:nat{i < len
                          index_is_item_is_mem_base tl item (i - 1)
 
 let index_is_item_is_mem (#a:eqtype) (l:list a)
-  : Lemma (ensures forall (item:a) (i:nat{i < length l}). index l i = item ==> mem i (item_index item l 0) = true)
+  : Lemma (ensures forall (item:a) (i:nat{i < length l}). index l i = item ==> mem i (item_indices item l 0) = true)
   = forall_intro_2 (index_is_item_is_mem_base l)
 
 let rec index_is_not_mem_is_not_item_base (#a:eqtype) (l:list a) (item:a) (i:nat{i < length l})
-  : Lemma (ensures mem i (item_index item l 0) = false ==> index l i <> item)
+  : Lemma (ensures mem i (item_indices item l 0) = false ==> index l i <> item)
   = match l with
     | [] -> ()
     | hd :: tl -> match i with 
@@ -233,15 +210,15 @@ let rec index_is_not_mem_is_not_item_base (#a:eqtype) (l:list a) (item:a) (i:nat
                          item_indices_one_and_item_indices_zero item tl i 1
 
 let index_is_not_mem_is_not_item_forall_i (#a:eqtype) (l:list a) (item:a)
-  : Lemma (ensures forall (i:nat{i < length l}). mem i (item_index item l 0) = false ==> index l i <> item)
+  : Lemma (ensures forall (i:nat{i < length l}). mem i (item_indices item l 0) = false ==> index l i <> item)
   = forall_intro (index_is_not_mem_is_not_item_base l item)
 
 let index_is_not_mem_is_not_item (#a:eqtype) (l:list a)
-  : Lemma (ensures forall (item:a) (i:nat{i < length l}). mem i (item_index item l 0) = false ==> index l i <> item)
+  : Lemma (ensures forall (item:a) (i:nat{i < length l}). mem i (item_indices item l 0) = false ==> index l i <> item)
   = forall_intro (index_is_not_mem_is_not_item_forall_i l)
 
 let rec index_is_mem_is_item_base (#a:eqtype) (l:list a) (item:a) (i:nat{i < length l})
-  : Lemma (ensures mem i (item_index item l 0) = true ==> index l i = item)
+  : Lemma (ensures mem i (item_indices item l 0) = true ==> index l i = item)
   = match l with
     | [] -> ()
     | hd :: tl -> match i with 
@@ -252,22 +229,22 @@ let rec index_is_mem_is_item_base (#a:eqtype) (l:list a) (item:a) (i:nat{i < len
                          item_indices_one_and_item_indices_zero item tl i 1
 
 let index_is_mem_is_item_forall_i (#a:eqtype) (l:list a) (item:a)
-  : Lemma (ensures forall (i:nat{i < length l}). mem i (item_index item l 0) = true ==> index l i = item)
+  : Lemma (ensures forall (i:nat{i < length l}). mem i (item_indices item l 0) = true ==> index l i = item)
   = forall_intro (index_is_mem_is_item_base l item)
 
 let index_is_mem_is_item (#a:eqtype) (l:list a)
-  : Lemma (ensures forall (item:a) (i:nat{i < length l}). mem i (item_index item l 0) = true ==> index l i = item)
+  : Lemma (ensures forall (item:a) (i:nat{i < length l}). mem i (item_indices item l 0) = true ==> index l i = item)
   = forall_intro (index_is_mem_is_item_forall_i l)
 
 let index_not_mem_not_item_not_item_not_mem (#a:eqtype) (l:list a)
-  : Lemma (ensures forall (item:a) (i:nat{i < length l}). mem i (item_index item l 0) = false <==> index l i <> item)
+  : Lemma (ensures forall (item:a) (i:nat{i < length l}). mem i (item_indices item l 0) = false <==> index l i <> item)
   = index_is_not_item_is_not_mem l;
     index_is_not_mem_is_not_item l
 
 let index_mem_item_item_mem (#a:eqtype) (l:list a)
-  : Lemma (ensures forall (item:a) (i:nat{i < length l}). mem i (item_index item l 0) = true <==> index l i = item)
-  = index_is_item_is_mem l;
-    index_is_mem_is_item l
+  : Lemma (ensures forall (item:a) (i:nat{i < length l}). mem i (item_indices item l 0) = true <==> index l i = item)
+  = index_is_mem_is_item l;
+    index_is_item_is_mem l
 
 let rec mem_index_element (#a:eqtype) (l:list a) (i:nat{i < length l})
   : Lemma (ensures mem (index l i) l = true)
@@ -281,28 +258,28 @@ let mem_index_element_forall (#a:eqtype) (l:list a)
   : Lemma (ensures forall (i:nat{i < length l}). mem (index l i) l = true)
   = forall_intro (mem_index_element l)
 
-let rec index_not_zero_not_first_element (#a:eqtype) (l:list a) (item:a) (m:nat) (i:nat{i < length (item_index item l m)})
-  : Lemma (requires length (item_index item l m) > 1)
+let rec index_not_zero_not_first_element (#a:eqtype) (l:list a) (item:a) (m:nat) (i:nat{i < length (item_indices item l m)})
+  : Lemma (requires length (item_indices item l m) > 1)
           (ensures 
-           (let indices = item_index item l m in
+           (let indices = item_indices item l m in
             i <> 0 ==> index indices i <> hd indices))
   = match l with 
     | [] -> ()
     | fst :: tl -> if fst = item 
                    then (
-                    assert(hd (item_index item l m) = m);
-                    assert(item_index item l m = m :: (item_index item tl (m + 1)));
+                    assert(hd (item_indices item l m) = m);
+                    assert(item_indices item l m = m :: (item_indices item tl (m + 1)));
                     match i with 
                     | 0 -> ()
-                    | _ -> mem_index_element (item_index item tl (m + 1)) (i - 1);
-                           item_indices_is_in_interval item tl (m + 1) (index (item_index item tl (m + 1)) (i - 1))
+                    | _ -> mem_index_element (item_indices item tl (m + 1)) (i - 1);
+                           item_indices_is_in_interval item tl (m + 1) (index (item_indices item tl (m + 1)) (i - 1))
                    )
                    else index_not_zero_not_first_element tl item (m + 1) i
 
 let rec hd_item_indices_is_min (#a:eqtype) (l:list a) (item:a) (i:nat) (m:nat)
-  : Lemma (requires length (item_index item l m) > 1)
+  : Lemma (requires length (item_indices item l m) > 1)
           (ensures 
-           (let indices = item_index item l m in 
+           (let indices = item_indices item l m in 
             mem i indices && i <> hd indices ==> i > hd indices))
   = match l with 
     | [] -> ()
@@ -320,7 +297,7 @@ let proof_subtraction (i:nat)
   = ()
 
 let rec item_indices_zero_is_item_indices_one_minus_one (#a:eqtype) (l:list a) (item:a) (m:nat)
-  : Lemma (ensures item_index item l m = map subtraction (item_index item l (m + 1)))
+  : Lemma (ensures item_indices item l m = map subtraction (item_indices item l (m + 1)))
   = match l with 
     | [] -> ()
     | hd :: tl -> item_indices_zero_is_item_indices_one_minus_one tl item (m + 1)
@@ -335,58 +312,82 @@ let rec item_map_subtraction (l:list nat) (i:nat{i < length l})
                   | 0 -> ()
                   | _ -> item_map_subtraction tl (i - 1)
 
-//item_indices item l m
-let rec indices_are_ordered_in_ascending_order (#a:eqtype) (l:list a) (item:a) (i:nat) (j:nat)
-  : Lemma (requires i < length (item_index item l 0) && j < length (item_index item l 0) && i < j)
+let rec indices_are_ordered_in_ascending_order_base (#a:eqtype) (l:list a) (item:a) 
+        (i:nat{i < length (item_indices item l 0)}) (j:nat{j < length (item_indices item l 0)})
+  : Lemma (requires i < j)
           (ensures 
-           (let indices = item_index item l 0 in
+           (let indices = item_indices item l 0 in
             index indices i < index indices j))
   = match l with 
     | [] -> ()
-    | fst :: tl -> match i with 
+    | fst :: tl -> let l' = item_indices item l 0 in 
+                   let l'' = item_indices item tl 1 in
+                   let l''' = item_indices item tl 0 in
+                   match i with 
                   | 0 -> if fst = item 
                          then (
-                          mem_index_element (item_index item tl 1) (j - 1);
-                          item_indices_is_in_interval item tl 1 (index (item_index item tl 1) (j - 1))
+                          mem_index_element l'' (j - 1);
+                          item_indices_is_in_interval item tl 1 (index l'' (j - 1))
                          )
                          else (
-                          if length (item_index item tl 1) < 2
+                          if length l'' < 2
                           then ()
                           else (
-                            mem_index_element (item_index item l 0) j;
+                            mem_index_element l' j;
                             index_not_zero_not_first_element l item 0 j;
-                            hd_item_indices_is_min l item (index (item_index item l 0) j) 0
+                            hd_item_indices_is_min l item (index l' j) 0
                           )
                          )
                   | _ -> item_indices_zero_is_item_indices_one_minus_one tl item 0;
-                         assert((item_index item tl 0) = map subtraction (item_index item tl 1));
+                         assert(l''' = map subtraction l'');
                          if fst = item
                          then (
-                          assert(index (item_index item l 0) i = index (item_index item tl 1) (i - 1));
-                          assert(index (item_index item l 0) j = index (item_index item tl 1) (j - 1));
-                          mem_index_element (item_index item tl 1) (i - 1);
-                          mem_index_element (item_index item tl 1) (j - 1);
-                          item_map_subtraction (item_index item tl 1) (i - 1);
-                          item_map_subtraction (item_index item tl 1) (j - 1);
-                          item_indices_is_in_interval item tl 1 (index (item_index item tl 1) (i - 1));
-                          item_indices_is_in_interval item tl 1 (index (item_index item tl 1) (j - 1));
-                          assert(index (item_index item tl 0) (i - 1) = (index (item_index item tl 1) (i - 1)) - 1);
-                          assert(index (item_index item tl 0) (j - 1) = (index (item_index item tl 1) (j - 1)) - 1);
-                          indices_are_ordered_in_ascending_order tl item (i - 1) (j - 1)
+                          assert(index l' i = index l'' (i - 1));
+                          assert(index l' j = index l'' (j - 1));
+                          mem_index_element l'' (i - 1);
+                          mem_index_element l'' (j - 1);
+                          item_map_subtraction l'' (i - 1);
+                          item_map_subtraction l'' (j - 1);
+                          item_indices_is_in_interval item tl 1 (index l'' (i - 1));
+                          item_indices_is_in_interval item tl 1 (index l'' (j - 1));
+                          assert(index l''' (i - 1) = (index l'' (i - 1)) - 1);
+                          assert(index l''' (j - 1) = (index l'' (j - 1)) - 1);
+                          indices_are_ordered_in_ascending_order_base tl item (i - 1) (j - 1)
                          )
                          else (
-                          assert(index (item_index item l 0) i = index (item_index item tl 1) i);
-                          assert(index (item_index item l 0) j = index (item_index item tl 1) j);
-                          mem_index_element (item_index item tl 1) i;
-                          mem_index_element (item_index item tl 1) j;
-                          item_map_subtraction (item_index item tl 1) i;
-                          item_map_subtraction (item_index item tl 1) j;
-                          item_indices_is_in_interval item tl 1 (index (item_index item tl 1) i);
-                          item_indices_is_in_interval item tl 1 (index (item_index item tl 1) j);
-                          assert(index (item_index item tl 0) i = (index (item_index item tl 1) i) - 1);
-                          assert(index (item_index item tl 0) j = (index (item_index item tl 1) j) - 1);
-                          indices_are_ordered_in_ascending_order tl item i j 
+                          assert(index l' i = index l'' i);
+                          assert(index l' j = index l'' j);
+                          mem_index_element l'' i;
+                          mem_index_element l'' j;
+                          item_map_subtraction l'' i;
+                          item_map_subtraction l'' j;
+                          item_indices_is_in_interval item tl 1 (index l'' i);
+                          item_indices_is_in_interval item tl 1 (index l'' j);
+                          assert(index l''' i = (index l'' i) - 1);
+                          assert(index l''' j = (index l'' j) - 1);
+                          indices_are_ordered_in_ascending_order_base tl item i j 
                          )
+
+let indices_are_ordered_in_ascending_order_implication (#a:eqtype) (l:list a) (item:a)
+  (i:nat{i < length (item_indices item l 0)}) (j:nat{j < length (item_indices item l 0)})
+  : Lemma (ensures i < j ==>
+           (let indices = item_indices item l 0 in
+            index indices i < index indices j))
+  = move_requires (indices_are_ordered_in_ascending_order_base l item i) j
+
+let indices_are_ordered_in_ascending_order (#a:eqtype) (l:list a) (item:a)
+  : Lemma (ensures forall (i:nat{i < length (item_indices item l 0)}) (j:nat{j < length (item_indices item l 0)}). 
+           i < j ==>
+           (let indices = item_indices item l 0 in
+            index indices i < index indices j))
+  = forall_intro_2 (indices_are_ordered_in_ascending_order_implication l item)
+
+let indices_are_ordered_in_ascending_order_forall_item (#a:eqtype) (l:list a)
+  : Lemma (ensures forall (item:a) (i:nat{i < length (item_indices item l 0)}) (j:nat{j < length (item_indices item l 0)}). 
+           i < j ==>
+           (let indices = item_indices item l 0 in
+            index indices i < index indices j))
+  = forall_intro (indices_are_ordered_in_ascending_order l)
 
 let rec last_is_length_l_minus_one (#a:eqtype) (l:list a)
   : Lemma (requires l <> [])
@@ -395,23 +396,23 @@ let rec last_is_length_l_minus_one (#a:eqtype) (l:list a)
     | [el] -> ()
     | hd :: tl -> last_is_length_l_minus_one tl
 
-let last_index_is_max_base (#a:eqtype) (item:a) (l:list a{item_index item l 0 <> []}) (i:nat{i < length (item_index item l 0) - 1})
+let last_index_is_max_base (#a:eqtype) (item:a) (l:list a{item_indices item l 0 <> []}) (i:nat{i < length (item_indices item l 0) - 1})
   : Lemma (ensures 
-           (let indices = item_index item l 0 in
+           (let indices = item_indices item l 0 in
             let j = (length indices) - 1 in
             index indices i < index indices j))
-  = indices_are_ordered_in_ascending_order l item i (length (item_index item l 0) - 1)
+  = indices_are_ordered_in_ascending_order_base l item i (length (item_indices item l 0) - 1)
 
-let last_index_is_max (#a:eqtype) (item:a) (l:list a{item_index item l 0 <> []}) 
-  : Lemma (ensures forall (i:nat{i < length (item_index item l 0) - 1}).
-           (let indices = item_index item l 0 in
+let last_index_is_max (#a:eqtype) (item:a) (l:list a{item_indices item l 0 <> []}) 
+  : Lemma (ensures forall (i:nat{i < length (item_indices item l 0) - 1}).
+           (let indices = item_indices item l 0 in
             let j = (length indices) - 1 in
             index indices i < index indices j))
   = forall_intro (last_index_is_max_base item l)
 
 let new_or_old (#a:eqtype) (c:a) (l:list a) : int
-  = if item_index c l 0 <> []
-    then last (item_index c l 0)
+  = if item_indices c l 0 <> []
+    then last (item_indices c l 0)
     else -1
 
 let rec mem_last_list (#a:eqtype) (l:list a)
@@ -423,27 +424,27 @@ let rec mem_last_list (#a:eqtype) (l:list a)
 
 let new_or_old_return_values (#a:eqtype) (l:list a) (item:a)
   : Lemma (ensures new_or_old item l = -1 || (new_or_old item l >= 0 && new_or_old item l < length l))
-  = if item_index item l 0 = []
+  = if item_indices item l 0 = []
     then ()
     else (
-      mem_last_list (item_index item l 0);
-      item_indices_is_in_interval item l 0 (last (item_index item l 0))
+      mem_last_list (item_indices item l 0);
+      item_indices_is_in_interval item l 0 (last (item_indices item l 0))
     )
 
 let rec not_new_or_old_empty_list (#a:eqtype) (l:list a) (item:a)
-  : Lemma (ensures new_or_old item l = -1 ==> item_index item l 0 = [])
+  : Lemma (ensures new_or_old item l = -1 ==> item_indices item l 0 = [])
   = match l with
     | [] -> ()
     | hd :: tl -> not_new_or_old_empty_list tl item 
 
 let rec empty_list_length_zero (#a:eqtype) (l:list a) (item:a)
-  : Lemma (ensures item_index item l 0 = [] ==> length (item_index item l 0) = 0)
+  : Lemma (ensures item_indices item l 0 = [] ==> length (item_indices item l 0) = 0)
   = match l with 
     | [] -> ()
     | hd :: tl -> empty_list_length_zero tl item
 
 let rec length_zero_count_zero (#a:eqtype) (l:list a) (item:a)
-  : Lemma (ensures length (item_index item l 0) = 0 ==> count item l = 0)
+  : Lemma (ensures length (item_indices item l 0) = 0 ==> count item l = 0)
   = match l with
     | [] -> ()
     | hd :: tl -> length_zero_count_zero tl item;
@@ -476,33 +477,33 @@ let rec new_or_old_not_item_base (#a:eqtype) (l:list a) (item:a) (i:nat{i < leng
                          count_zero_mem_false l item;
                          mem_false_not_item l item i
 
-let new_or_old_not_item (#a:eqtype) (l:list a)
-  : Lemma (ensures forall (item:a) (i:nat{i < length l}). new_or_old item l = -1 ==> index l i <> item)
-  = forall_intro_2 (new_or_old_not_item_base l)   
+let new_or_old_not_item (#a:eqtype) (l:list a) (item:a)
+  : Lemma (ensures forall (i:nat{i < length l}). new_or_old item l = -1 ==> index l i <> item)
+  = forall_intro (new_or_old_not_item_base l item)   
 
 let rec new_or_old_not_empty_list (#a:eqtype) (l:list a)
-  : Lemma (ensures forall (item:a). new_or_old item l <> -1 ==> item_index item l 0 <> [])
+  : Lemma (ensures forall (item:a). new_or_old item l <> -1 ==> item_indices item l 0 <> [])
   = match l with
     | [] -> ()
     | hd :: tl -> new_or_old_not_empty_list tl
 
-let rec not_empty_list_length_greater_than_zero_base (#a:eqtype) (l:list a) (item:a)
-  : Lemma (ensures item_index item l 0 <> [] ==> mem (last (item_index item l 0)) (item_index item l 0) = true)
+let rec not_empty_list_mem_is_true_base (#a:eqtype) (l:list a) (item:a)
+  : Lemma (ensures item_indices item l 0 <> [] ==> mem (last (item_indices item l 0)) (item_indices item l 0) = true)
   = match l with
     | [] -> ()
-    | hd :: tl -> not_empty_list_length_greater_than_zero_base tl item;
-                  if item_index item l 0 <> []
-                  then mem_last_list (item_index item l 0)
+    | hd :: tl -> not_empty_list_mem_is_true_base tl item;
+                  if item_indices item l 0 <> []
+                  then mem_last_list (item_indices item l 0)
                   else ()
 
-let not_empty_list_length_greater_than_zero (#a:eqtype) (l:list a)
-  : Lemma (ensures forall (item:a). item_index item l 0 <> [] ==> mem (last (item_index item l 0)) (item_index item l 0) = true)
-  = forall_intro (not_empty_list_length_greater_than_zero_base l)
+let not_empty_list_mem_is_true (#a:eqtype) (l:list a)
+  : Lemma (ensures forall (item:a). item_indices item l 0 <> [] ==> mem (last (item_indices item l 0)) (item_indices item l 0) = true)
+  = forall_intro (not_empty_list_mem_is_true_base l)
  
 let mem_index_is_item (#a:eqtype) (item:a) (l:list a)
-  : Lemma (requires item_index item l 0 <> [] && last (item_index item l 0) < length l)
-          (ensures mem (last (item_index item l 0)) (item_index item l 0) = true ==> index l (last (item_index item l 0)) = item)
-  = mem_last_list (item_index item l 0);
+  : Lemma (requires item_indices item l 0 <> [] && last (item_indices item l 0) < length l)
+          (ensures mem (last (item_indices item l 0)) (item_indices item l 0) = true ==> index l (last (item_indices item l 0)) = item)
+  = mem_last_list (item_indices item l 0);
     index_is_mem_is_item l
 
 let rec index_plus_one_base (#a:eqtype) (l:list a) (item:a) (el:a) (i:nat{i < length l})
@@ -540,61 +541,47 @@ let rec mem_list_exists_index (#a:eqtype) (l:list a) (item:a)
                     exists_tl_exists_tl_plus_hd tl item hd
                   )
 
-let index_in_list_is_less_than_last_base (#a:eqtype) (item:a) (l:list a{item_index item l 0 <> []}) (x:nat)
-  : Lemma (ensures mem x (item_index item l 0) = true ==> x <= last (item_index item l 0))
-  = mem_list_exists_index (item_index item l 0) x;
+let index_in_list_is_less_than_last_base (#a:eqtype) (item:a) (l:list a{item_indices item l 0 <> []}) (x:nat)
+  : Lemma (ensures mem x (item_indices item l 0) = true ==> x <= last (item_indices item l 0))
+  = mem_list_exists_index (item_indices item l 0) x;
     last_index_is_max item l;
-    last_is_length_l_minus_one (item_index item l 0)
+    last_is_length_l_minus_one (item_indices item l 0)
 
-let index_in_list_is_less_than_last (#a:eqtype) (item:a) (l:list a{item_index item l 0 <> []})
-  : Lemma (ensures forall (i:nat). mem i (item_index item l 0) = true ==> i <= last (item_index item l 0))
+let index_in_list_is_less_than_last (#a:eqtype) (item:a) (l:list a{item_indices item l 0 <> []})
+  : Lemma (ensures forall (i:nat). mem i (item_indices item l 0) = true ==> i <= last (item_indices item l 0))
   = forall_intro (index_in_list_is_less_than_last_base item l)
 
-let index_greater_than_last_not_item (#a:eqtype) (item:a) (l:list a{item_index item l 0 <> []}) (i:nat{i < length l})
-  : Lemma (ensures i > (last (item_index item l 0)) ==> index l i <> item)
+let index_greater_than_last_not_item (#a:eqtype) (item:a) (l:list a{item_indices item l 0 <> []}) (i:nat{i < length l})
+  : Lemma (ensures i > (last (item_indices item l 0)) ==> index l i <> item)
   = index_is_not_mem_is_not_item_forall_i l item;
     index_in_list_is_less_than_last item l
 
-let mem_index_is_item_last_indices_are_not_item_base (#a:eqtype) (item:a) (l:list a{item_index item l 0 <> []}) (i:nat{i > (last (item_index item l 0)) && i < length l})
-  : Lemma (ensures mem (last (item_index item l 0)) (item_index item l 0) = true ==> index l i <> item)
+let mem_index_is_item_last_indices_are_not_item_base (#a:eqtype) (item:a) (l:list a{item_indices item l 0 <> []}) (i:nat{i > (last (item_indices item l 0)) && i < length l})
+  : Lemma (ensures mem (last (item_indices item l 0)) (item_indices item l 0) = true ==> index l i <> item)
   = index_greater_than_last_not_item item l i
 
-let mem_index_is_item_last_indices_are_not_item (#a:eqtype) (item:a) (l:list a{item_index item l 0 <> []})
-  : Lemma (ensures mem (last (item_index item l 0)) (item_index item l 0) = true ==> (forall (i:nat{i > (last (item_index item l 0)) && i < length l}). index l i <> item))
+let mem_index_is_item_last_indices_are_not_item (#a:eqtype) (item:a) (l:list a{item_indices item l 0 <> []})
+  : Lemma (ensures mem (last (item_indices item l 0)) (item_indices item l 0) = true ==> (forall (i:nat{i > (last (item_indices item l 0)) && i < length l}). index l i <> item))
   = forall_intro (index_greater_than_last_not_item item l)
 
 let mem_index_is_item_gives_correct_result (#a:eqtype) (l:list a) (item:a)
-  : Lemma (requires item_index item l 0 <> [] && (last (item_index item l 0)) < length l)
-          (ensures mem (last (item_index item l 0)) (item_index item l 0) = true ==> index l (last (item_index item l 0)) = item /\ 
-          (forall (i:nat{i > (last (item_index item l 0)) && i < length l}). index l i <> item))
+  : Lemma (requires item_indices item l 0 <> [] && (last (item_indices item l 0)) < length l)
+          (ensures mem (last (item_indices item l 0)) (item_indices item l 0) = true ==> index l (last (item_indices item l 0)) = item /\ 
+          (forall (i:nat{i > (last (item_indices item l 0)) && i < length l}). index l i <> item))
   = mem_index_is_item item l;
     mem_index_is_item_last_indices_are_not_item item l
 
-let new_or_old_not_empty_list_correct_item_base (#a:eqtype) (l:list a) (item:a)
-  : Lemma (requires item_index item l 0 <> [] && last (item_index item l 0) < length l)
-          (ensures new_or_old item l <> -1 ==> index l (last (item_index item l 0)) = item /\ 
-          (forall (i:nat{i > (last (item_index item l 0)) && i < length l}). index l i <> item))
+let new_or_old_not_empty_list_correct_item (#a:eqtype) (l:list a) (item:a)
+  : Lemma (requires item_indices item l 0 <> [] && last (item_indices item l 0) < length l)
+          (ensures new_or_old item l <> -1 ==> index l (last (item_indices item l 0)) = item /\ 
+          (forall (i:nat{i > (last (item_indices item l 0)) && i < length l}). index l i <> item))
   = new_or_old_not_empty_list l;
-    not_empty_list_length_greater_than_zero l;
+    not_empty_list_mem_is_true l;
     mem_index_is_item_gives_correct_result l item
-
-let new_or_old_not_empty_list_correct_item_implication (#a:eqtype) (l:list a) (item:a)
-  : Lemma (ensures (item_index item l 0 <> [] && last (item_index item l 0) < length l) ==> 
-                   (new_or_old item l <> -1 ==> index l (last (item_index item l 0)) = item /\
-                   (forall (i:nat{i > (last (item_index item l 0)) && i < length l}). index l i <> item)))
-  = if item_index item l 0 = []
-    then ()
-    else (
-      mem_last_list (item_index item l 0);
-      item_indices_is_in_interval_forall item l 0;
-      assert(item_index item l 0 <> [] && last (item_index item l 0) < length l);
-      // move_requires (new_or_old_not_empty_list_correct_item_base l) item
-      admit()
-    )
     
-val update_bc (a:list english_letters) (p:list english_letters) : list int
-let rec update_bc a p = 
-    match a with 
+let rec update_bc (a:list english_letters) (p:list english_letters) 
+  : list int
+  = match a with 
     | [] -> []
     | hd :: tl -> (new_or_old hd p) :: update_bc tl p
 
@@ -604,8 +591,9 @@ let rec update_bc_length_is_initial_list_length (l:list english_letters) (p:list
     | [] -> ()
     | hd :: tl -> update_bc_length_is_initial_list_length tl p
 
-let rec update_bc_has_index_minusone_if_letter_is_not_in_pattern_base (l:list english_letters) (p:list english_letters)
-                                                                      (i:nat{i < length l && i < length (update_bc l p)}) (j:nat{j < length p})
+let rec update_bc_for_minusone_base (l:list english_letters) (p:list english_letters)
+                                    (i:nat{i < length l && i < length (update_bc l p)}) 
+                                    (j:nat{j < length p})
   : Lemma (ensures 
            (let l' = update_bc l p in
             index l' i = -1 ==> index p j <> index l i))
@@ -617,27 +605,27 @@ let rec update_bc_has_index_minusone_if_letter_is_not_in_pattern_base (l:list en
                           assert(index (update_bc l p) i = new_or_old fst p);
                           assert(fst = index l i);
                           new_or_old_not_item_base p fst j;
-                          assert(new_or_old fst p = - 1 ==> index p j <> fst)
-                   | _ -> update_bc_has_index_minusone_if_letter_is_not_in_pattern_base tl p (i - 1) j
+                          assert(new_or_old fst p = -1 ==> index p j <> fst)
+                   | _ -> update_bc_for_minusone_base tl p (i - 1) j
 
-let update_bc_has_index_minusone_if_letter_is_not_in_pattern_forall_j (l:list english_letters) 
-                                                                      (p:list english_letters) 
-                                                                      (i:nat{i < length l && i < length (update_bc l p)})
+let update_bc_for_minusone_forall_j (l:list english_letters) 
+                                    (p:list english_letters) 
+                                    (i:nat{i < length l && i < length (update_bc l p)})
   : Lemma (ensures forall (j:nat{j < length p}).  
            (let l' = update_bc l p in
             index l' i = -1 ==> index p j <> index l i))
-  = forall_intro (update_bc_has_index_minusone_if_letter_is_not_in_pattern_base l p i)
+  = forall_intro (update_bc_for_minusone_base l p i)
 
-let update_bc_has_index_minusone_if_letter_is_not_in_pattern (l:list english_letters) (p:list english_letters)
+let update_bc_for_minusone (l:list english_letters) (p:list english_letters)
   : Lemma (ensures forall (i:nat{i < length l && i < length (update_bc l p)}). (forall (j:nat{j < length p}).  
            (let l' = update_bc l p in
             index l' i = -1 ==> index p j <> index l i)))
-  = forall_intro (update_bc_has_index_minusone_if_letter_is_not_in_pattern_forall_j l p)
+  = forall_intro (update_bc_for_minusone_forall_j l p)
 
-let rec update_bc_has_correct_index_if_letter_is_in_pattern_base (l:list english_letters)
-                                                                 (p:list english_letters)
-                                                                 (i:nat{i < length l && i < length (update_bc l p)}) 
-                                                                 (j:nat{j < length p})
+let rec update_bc_for_nat_base (l:list english_letters)
+                               (p:list english_letters)
+                               (i:nat{i < length l && i < length (update_bc l p)}) 
+                               (j:nat{j < length p})
   : Lemma (ensures 
            (let l' = update_bc l p in
             index l' i = j ==> index p j = index l i /\ (forall (i':nat{i' > j && i' < length p}). index p i' <> index l i)))
@@ -650,30 +638,30 @@ let rec update_bc_has_correct_index_if_letter_is_in_pattern_base (l:list english
                           assert(fst = index l i);
                           if j = new_or_old fst p
                           then (
-                            if item_index (index l i) l 0 <> []
+                            if item_indices (index l i) l 0 <> []
                             then (
-                              item_indices_is_in_interval (index l i) l 0 (last (item_index (index l i) l 0));
-                              new_or_old_not_empty_list_correct_item_base p fst
+                              item_indices_is_in_interval (index l i) l 0 (last (item_indices (index l i) l 0));
+                              new_or_old_not_empty_list_correct_item p fst
                             )
                             else ()
                           )
                           else ()
-                   | _ -> update_bc_has_correct_index_if_letter_is_in_pattern_base tl p (i - 1) j
+                   | _ -> update_bc_for_nat_base tl p (i - 1) j
 
-let update_bc_has_correct_index_if_letter_is_in_pattern_forall_j (l:list english_letters) 
-                                                                 (p:list english_letters)
-                                                                 (i:nat{i < length l && i < length (update_bc l p)})
+let update_bc_for_nat_forall_j (l:list english_letters) 
+                               (p:list english_letters)
+                               (i:nat{i < length l && i < length (update_bc l p)})
   : Lemma (ensures 
            (let l' = update_bc l p in forall (j:nat{j < length p}).
             index l' i = j ==> index p j = index l i /\ (forall (i':nat{i' > j && i' < length p}). index p i' <> index l i)))
-  = forall_intro (update_bc_has_correct_index_if_letter_is_in_pattern_base l p i)
+  = forall_intro (update_bc_for_nat_base l p i)
 
-let update_bc_has_correct_index_if_letter_is_in_pattern (l:list english_letters) (p:list english_letters)
+let update_bc_for_nat (l:list english_letters) (p:list english_letters)
   : Lemma (ensures 
            (let l' = update_bc l p in forall (i:nat{i < length l && i < length (update_bc l p)}) (j:nat{j < length p}).
             index l' i = j ==> index p j = index l i /\ 
             (forall (i':nat{i' > j && i' < length p}). index p i' <> index l i)))
-  = forall_intro (update_bc_has_correct_index_if_letter_is_in_pattern_forall_j l p)
+  = forall_intro (update_bc_for_nat_forall_j l p)
 
 let rec update_bc_has_values_in_interval (l:list english_letters) (p:list english_letters) (i:nat{i < length (update_bc l p)})
   : Lemma (ensures 
@@ -691,7 +679,7 @@ let update_bc_has_index_minusone_if_letter_is_not_in_pattern_for_alphabet ()
   : Lemma (ensures forall (i:nat{i < length alphabet && i < length (update_bc alphabet pattern)}). (forall (j:nat{j < length pattern}).  
            (let l' = update_bc alphabet pattern in
             index l' i = -1 ==> index pattern j <> index alphabet i)))
-  = update_bc_has_index_minusone_if_letter_is_not_in_pattern alphabet pattern
+  = update_bc_for_minusone alphabet pattern
 
 let update_bc_has_correct_index_if_letter_is_in_pattern_for_alphabet ()
   : Lemma (ensures 
@@ -699,7 +687,7 @@ let update_bc_has_correct_index_if_letter_is_in_pattern_for_alphabet ()
             (i:nat{i < length alphabet && i < length (update_bc alphabet pattern)}) (j:nat{j < length pattern}).
             index l' i = j ==> index pattern j = index alphabet i /\ 
             (forall (i':nat{i' > j && i' < length pattern}). index pattern i' <> index alphabet i)))
-  = update_bc_has_correct_index_if_letter_is_in_pattern alphabet pattern
+  = update_bc_for_nat alphabet pattern
 
 let final_bc_has_same_length_as_alphabet () 
   : Lemma (ensures length final_bc = length alphabet)
@@ -794,74 +782,44 @@ let minimum_returns_correct_result ()
   : Lemma (ensures forall (a:int) (b:int). minimum a b = a ==> a <= b)
   = forall_intro_2 minimum_returns_correct_result_base
 
-let item_index_of_t_in_alphabet (t:list english_letters) (i:nat{i < length t})
-  : Lemma (ensures item_index (index t i) alphabet 0 <> [])
-  = match index t i with 
-    | A -> assert(index t i = index alphabet 0)
-    | B -> assert(index t i = index alphabet 1)
-
-let last_is_less_than_bc (t:list english_letters) (p:list english_letters{length p <= length t}) (i:nat{i < length t}) 
-  : Lemma (requires item_index (index t i) alphabet 0 <> [])
-          (ensures last (item_index (index t i) alphabet 0) < length (update_bc alphabet p))
-  = mem_last_list (item_index (index t i) alphabet 0);
-    update_bc_length_is_initial_list_length alphabet p;
-    item_indices_is_in_interval (index t i) alphabet 0 (last (item_index (index t i) alphabet 0))
-
-val boyer_moore (t:list english_letters) (p:list english_letters{length p <= length t}) (k:nat{k <= length p}) (i:nat) 
-    : Tot (result:int{result >= -1}) 
-    (decreases %[(if i < length t - length p + 1 then length t - length p + 1 - i else 0); length p - k])
-let rec boyer_moore t p k i =
-    let m = length p in
+let rec boyer_moore_horspool (t:list english_letters) (p:list english_letters{length p <= length t}) (k:nat{k <= length p}) (i:nat) 
+  : Tot (result:int{result >= -1}) 
+  (decreases %[(if i < length t - length p + 1 then length t - length p + 1 - i else 0); length p - k]) 
+  = let m = length p in
     let n = length t in
     if k = m then i
     else if i > n - m then -1 
     else (
       if index t (i + m - 1 - k) = index p (m - 1 - k)
-      then boyer_moore t p (k + 1) i
+      then boyer_moore_horspool t p (k + 1) i
       else (
-        item_index_of_t_in_alphabet t (i + m - 1 - k);
-        last_is_less_than_bc t p (i + m - 1 - k);
-        let shiftbc = m - k - 1 - index (update_bc alphabet p) (last (item_index (index t (i + m - 1 - k)) alphabet 0)) in
+        update_bc_length_is_initial_list_length alphabet p;
+        mem_last_list (item_indices (index t (i + m - 1 - k)) alphabet 0);
+        item_indices_is_in_interval_forall alphabet 0 (index t (i + m - 1 - k));
+        let shiftbc = m - k - 1 - index (update_bc alphabet p) (last (item_indices (index t (i + m - 1 - k)) alphabet 0)) in
         let value = i + (maximum 1 shiftbc) in
-        boyer_moore t p 0 value
+        boyer_moore_horspool t p 0 value
       ) 
     )
 
-//don't know if usefull 
-let rec length_init_list_is_length_list_minus_one (l:list english_letters)
-  : Lemma (requires l <> [])
-          (ensures length (init l) = length l - 1)
-  = match l with 
-    | [el] -> ()
-    | hd :: tl -> length_init_list_is_length_list_minus_one tl
-
-//don't know if usefull
-let rec p_less_than_t_then_init_p_less_than_t (t:list english_letters) (p:list english_letters{length p <= length t})
-  : Lemma (requires length p > 0)
-          (ensures length p <= length t ==> length (init p) <= length t)
-  = match p with 
-    | [el] -> ()
-    | hd :: tl -> length_init_list_is_length_list_minus_one p;
-                  p_less_than_t_then_init_p_less_than_t t tl
-
-let boyer_moore_result_base (t:list english_letters) (p:list english_letters{length p <= length t}) 
+let bmh_result_base (t:list english_letters) (p:list english_letters{length p <= length t}) 
                             (k:nat{k < length p}) (i:nat{i <= length t - length p})
-  : Lemma (requires boyer_moore t p k i = boyer_moore t p (length p) i)
-          (ensures boyer_moore t p k i = i)
+  : Lemma (requires boyer_moore_horspool t p k i = boyer_moore_horspool t p (length p) i)
+          (ensures boyer_moore_horspool t p k i = i)
   = ()
 
-let boyer_moore_result_implication (t:list english_letters) (p:list english_letters{length p <= length t}) 
+let bmh_result_implication (t:list english_letters) (p:list english_letters{length p <= length t}) 
                                    (k:nat{k < length p}) (i:nat{i <= length t - length p})
-  : Lemma (ensures boyer_moore t p k i = boyer_moore t p (length p) i ==> boyer_moore t p k i = i)
-  = move_requires (boyer_moore_result_base t p k) i
+  : Lemma (ensures boyer_moore_horspool t p k i = boyer_moore_horspool t p (length p) i ==> boyer_moore_horspool t p k i = i)
+  = move_requires (bmh_result_base t p k) i
 
-let boyer_moore_result (t:list english_letters) (p:list english_letters{length p <= length t})
-  : Lemma (ensures forall (k:nat{k < length p}) (i:nat{i <= length t - length p}). boyer_moore t p k i = boyer_moore t p (length p) i ==> boyer_moore t p k i = i)
-  = forall_intro_2 (boyer_moore_result_implication t p)
+let bmh_result (t:list english_letters) (p:list english_letters{length p <= length t})
+  : Lemma (ensures forall (k:nat{k < length p}) (i:nat{i <= length t - length p}). boyer_moore_horspool t p k i = boyer_moore_horspool t p (length p) i ==> boyer_moore_horspool t p k i = i)
+  = forall_intro_2 (bmh_result_implication t p)
 
-let rec boyer_moore_value_comparison (t:list english_letters) (p:list english_letters{length p <= length t}) 
+let rec bmh_value_comparison (t:list english_letters) (p:list english_letters{length p <= length t}) 
                                      (k:nat{k <= length p}) (i:nat)
-  : Lemma (ensures boyer_moore t p k i <> boyer_moore t p (length p) i ==> boyer_moore t p k i > i || boyer_moore t p k i = -1)
+  : Lemma (ensures boyer_moore_horspool t p k i <> boyer_moore_horspool t p (length p) i ==> boyer_moore_horspool t p k i > i || boyer_moore_horspool t p k i = -1)
           (decreases %[(if i < length t - length p + 1 then length t - length p + 1 - i else 0); length p - k])
   = let m = length p in 
     let n = length t in 
@@ -872,39 +830,41 @@ let rec boyer_moore_value_comparison (t:list english_letters) (p:list english_le
       then ()
       else (
         if index t (i + m - 1 - k) = index p (m - 1 - k) 
-        then boyer_moore_value_comparison t p (k + 1) i
+        then bmh_value_comparison t p (k + 1) i
         else (
-          item_index_of_t_in_alphabet t (i + m - 1 - k);
-          last_is_less_than_bc t p (i + m - 1 - k);
-          let shiftbc = m - k - 1 - index (update_bc alphabet p) (last (item_index (index t (i + m - 1 - k)) alphabet 0)) in
+          update_bc_length_is_initial_list_length alphabet p;
+          mem_last_list (item_indices (index t (i + length p - 1 - k)) alphabet 0);
+          item_indices_is_in_interval_forall alphabet 0 (index t (i + length p - 1 - k));
+          let shiftbc = m - k - 1 - index (update_bc alphabet p) (last (item_indices (index t (i + m - 1 - k)) alphabet 0)) in
           let value = i + (maximum 1 shiftbc) in
-          boyer_moore_value_comparison t p 0 value
+          bmh_value_comparison t p 0 value
         )
       )
     )
 
 let k_to_m_then_index_is_equal (t:list english_letters) (p:list english_letters{length p <= length t}) 
                                    (k:nat{k < length p}) (i:nat{i <= length t - length p})
-  : Lemma (requires boyer_moore t p k i = boyer_moore t p (length p) i)
+  : Lemma (requires boyer_moore_horspool t p k i = boyer_moore_horspool t p (length p) i)
           (ensures index t (i + length p - 1 - k) = index p (length p - 1 - k))
-  = item_index_of_t_in_alphabet t (i + length p - 1 - k);
-    last_is_less_than_bc t p (i + length p - 1 - k);
+  = update_bc_length_is_initial_list_length alphabet p;
+    mem_last_list (item_indices (index t (i + length p - 1 - k)) alphabet 0);
+    item_indices_is_in_interval_forall alphabet 0 (index t (i + length p - 1 - k));
     let bc = update_bc alphabet p in
-    let shiftbc = length p - k - 1 - index bc (last (item_index (index t (i + length p - 1 - k)) alphabet 0)) in
+    let shiftbc = length p - k - 1 - index bc (last (item_indices (index t (i + length p - 1 - k)) alphabet 0)) in
     let value = i + (maximum 1 shiftbc) in
     if index t (i + length p - 1 - k) <> index p (length p - 1 - k)
     then (
-      assert(index t (i + length p - 1 - k) <> index p (length p - 1 - k) ==> boyer_moore t p k i = boyer_moore t p 0 value);
-      boyer_moore_value_comparison t p 0 value;
-      assert(boyer_moore t p 0 value > i || boyer_moore t p 0 value = -1);
-      assert(boyer_moore t p 0 value <> boyer_moore t p (length p) i)
+      assert(index t (i + length p - 1 - k) <> index p (length p - 1 - k) ==> boyer_moore_horspool t p k i = boyer_moore_horspool t p 0 value);
+      bmh_value_comparison t p 0 value;
+      assert(boyer_moore_horspool t p 0 value > i || boyer_moore_horspool t p 0 value = -1);
+      assert(boyer_moore_horspool t p 0 value <> boyer_moore_horspool t p (length p) i)
     )
     else ()
 
 let rec k_to_m_then_k'_index_is_equal_base (t:list english_letters) (p:list english_letters{length p <= length t}) 
                                       (k:nat{k < length p}) (i:nat{i <= length t - length p})
                                       (k':nat{k' >= k && k' < length p})
-  : Lemma (requires boyer_moore t p k i = boyer_moore t p (length p) i)
+  : Lemma (requires boyer_moore_horspool t p k i = boyer_moore_horspool t p (length p) i)
           (ensures index t (i + length p - 1 - k') = index p (length p - 1 - k'))
           (decreases length p - k)
   = k_to_m_then_index_is_equal t p k i;
@@ -912,25 +872,25 @@ let rec k_to_m_then_k'_index_is_equal_base (t:list english_letters) (p:list engl
     then ()
     else if k = k' then ()
     else (
-      assert(index t (i + length p - 1 - k) = index p (length p - 1 - k) ==> boyer_moore t p k i = boyer_moore t p (k + 1) i);
+      assert(index t (i + length p - 1 - k) = index p (length p - 1 - k) ==> boyer_moore_horspool t p k i = boyer_moore_horspool t p (k + 1) i);
       k_to_m_then_k'_index_is_equal_base t p (k + 1) i k'
     )
 
 let k_to_m_then_k'_index_is_equal_implication (t:list english_letters) (p:list english_letters{length p <= length t}) 
                                               (k:nat{k < length p}) (i:nat{i <= length t - length p})
                                               (k':nat{k' >= k && k' < length p})
-  : Lemma (ensures boyer_moore t p k i = boyer_moore t p (length p) i ==> index t (i + length p - 1 - k') = index p (length p - 1 - k'))
+  : Lemma (ensures boyer_moore_horspool t p k i = boyer_moore_horspool t p (length p) i ==> index t (i + length p - 1 - k') = index p (length p - 1 - k'))
   = move_requires (k_to_m_then_k'_index_is_equal_base t p k i) k'
 
 let k_to_m_then_k'_index_is_equal_forall_k' (t:list english_letters) (p:list english_letters{length p <= length t}) 
                                             (k:nat{k < length p}) (i:nat{i <= length t - length p})
-  : Lemma (ensures boyer_moore t p k i = boyer_moore t p (length p) i ==> 
+  : Lemma (ensures boyer_moore_horspool t p k i = boyer_moore_horspool t p (length p) i ==> 
            (forall (k':nat{k' >= k && k' < length p}). index t (i + length p - 1 - k') = index p (length p - 1 - k')))
   = forall_intro (k_to_m_then_k'_index_is_equal_implication t p k i)
 
 let k_to_m_then_k'_index_is_equal (t:list english_letters) (p:list english_letters{length p <= length t}) 
   : Lemma (ensures forall (k:nat{k < length p}) (i:nat{i <= length t - length p}). 
-           boyer_moore t p k i = boyer_moore t p (length p) i ==> 
+           boyer_moore_horspool t p k i = boyer_moore_horspool t p (length p) i ==> 
            (forall (k':nat{k' >= k && k' < length p}). index t (i + length p - 1 - k') = index p (length p - 1 - k')))
   = forall_intro_3 (k_to_m_then_k'_index_is_equal_implication t p)
 
@@ -953,7 +913,7 @@ let convert_from_x_to_j (p:list english_letters) (i:nat)
 
 let zero_to_m_then_belongs_true (t:list english_letters) (p:list english_letters{length p <= length t}) 
                                 (i:nat{i <= length t - length p})
-  : Lemma (requires boyer_moore t p 0 i = boyer_moore t p (length p) i)
+  : Lemma (requires boyer_moore_horspool t p 0 i = boyer_moore_horspool t p (length p) i)
           (ensures belongs t p i = true)
   = if length p > 0 
     then (
@@ -966,143 +926,144 @@ let zero_to_m_then_belongs_true (t:list english_letters) (p:list english_letters
     )
     else ()
 
-let zero_to_k_than_all_indices_are_equal (t:list english_letters) (p:list english_letters{length p <= length t}) 
+// #push-options "--split_queries always"
+let zero_to_k_then_all_indices_are_equal (t:list english_letters) (p:list english_letters{length p <= length t}) 
                                          (k:nat{k < length p}) (i:nat{i <= length t - length p})
-  : Lemma (requires //boyer_moore t p 0 i = boyer_moore t p k i /\
-                    (forall (k':nat{k' < k}). index t (i + length p - 1 - k') = index p (length p - 1 - k')) /\
+  : Lemma (requires (forall (k':nat{k' < k}). index t (i + length p - 1 - k') = index p (length p - 1 - k')) /\
                     index t (i + length p - 1 - k) = index p (length p - 1 - k))
-          (ensures boyer_moore t p k i = boyer_moore t p (k + 1) i /\
+          (ensures boyer_moore_horspool t p k i = boyer_moore_horspool t p (k + 1) i /\
                    (forall (k':nat{k' < k + 1}). index t (i + length p - 1 - k') = index p (length p - 1 - k')))
   = ()
+// #pop-options
 
-let rec boyer_moore_not_equal_indices_then_increase_i (t:list english_letters) (p:list english_letters{length p <= length t}) 
+let rec bmh_not_equal_indices_then_increase_i (t:list english_letters) (p:list english_letters{length p <= length t}) 
                                                       (k:nat{k < length p}) (i:nat{i <= length t - length p})
-  : Lemma (requires boyer_moore t p k i <> boyer_moore t p (length p) i)
+  : Lemma (requires boyer_moore_horspool t p k i <> boyer_moore_horspool t p (length p) i)
           (ensures exists (k':nat{k' >= k && k' < length p}). index t (i + length p - 1 - k') <> index p (length p - 1 - k'))
           (decreases length p - k)
   = if index t (i + length p - 1 - k) = index p (length p - 1 - k)
-    then boyer_moore_not_equal_indices_then_increase_i t p (k + 1) i 
+    then bmh_not_equal_indices_then_increase_i t p (k + 1) i 
     else ()
 
-let from_zero_to_i_boyer_moore_does_not_return_i_base (t:list english_letters) (p:list english_letters{length p <= length t}) 
+let from_zero_to_i_bmh_does_not_return_i_base (t:list english_letters) (p:list english_letters{length p <= length t}) 
                                                       (i:nat{i <= length t - length p}) (i':nat{i' < i})
-  : Lemma (requires boyer_moore t p 0 0 = boyer_moore t p 0 i)
-          (ensures boyer_moore t p 0 i' <> boyer_moore t p (length p) i')
-  = admit()
+  : Lemma (requires forall (j:nat{j < i}). boyer_moore_horspool t p 0 j <> j)
+          (ensures boyer_moore_horspool t p 0 i' <> boyer_moore_horspool t p (length p) i')
+  = ()
 
-let from_zero_to_i_boyer_moore_does_not_return_i_implication (t:list english_letters) (p:list english_letters{length p <= length t}) 
+let from_zero_to_i_bmh_does_not_return_i_implication (t:list english_letters) (p:list english_letters{length p <= length t}) 
                                                              (i:nat{i <= length t - length p}) (i':nat{i' < i})
-  : Lemma (ensures boyer_moore t p 0 0 = boyer_moore t p 0 i ==> boyer_moore t p 0 i' <> boyer_moore t p (length p) i')
-  = move_requires (from_zero_to_i_boyer_moore_does_not_return_i_base t p i) i'
+  : Lemma (ensures (forall (j:nat{j < i}). boyer_moore_horspool t p 0 j <> j) ==> boyer_moore_horspool t p 0 i' <> boyer_moore_horspool t p (length p) i')
+  = move_requires (from_zero_to_i_bmh_does_not_return_i_base t p i) i'
 
-let from_zero_to_i_boyer_moore_does_not_return_i (t:list english_letters) (p:list english_letters{length p <= length t}) 
+let from_zero_to_i_bmh_does_not_return_i (t:list english_letters) (p:list english_letters{length p <= length t}) 
                                                  (i:nat{i <= length t - length p}) 
-  : Lemma (ensures forall (i':nat{i' < i}). boyer_moore t p 0 0 = boyer_moore t p 0 i ==> boyer_moore t p 0 i' <> boyer_moore t p (length p) i')
-  = forall_intro (from_zero_to_i_boyer_moore_does_not_return_i_implication t p i)
+  : Lemma (ensures forall (i':nat{i' < i}). (forall (j:nat{j < i}). boyer_moore_horspool t p 0 j <> j) ==> boyer_moore_horspool t p 0 i' <> boyer_moore_horspool t p (length p) i')
+  = forall_intro (from_zero_to_i_bmh_does_not_return_i_implication t p i)
 
-let from_zero_to_i_belongs_is_false (t:list english_letters) (p:list english_letters{length p <= length t}) 
-                                    (i:nat{i <= length t - length p}) (i':nat{i' < i})
-  : Lemma (requires boyer_moore t p 0 0 = boyer_moore t p 0 i)
+let from_zero_to_i_belongs_is_false_base (t:list english_letters) (p:list english_letters{length p <= length t}) 
+                                         (i:nat{i <= length t - length p}) (i':nat{i' < i})
+  : Lemma (requires forall (j:nat{j < i}). boyer_moore_horspool t p 0 j <> j)
           (ensures belongs t p i' = false)
-  = from_zero_to_i_boyer_moore_does_not_return_i t p i;
-    boyer_moore_not_equal_indices_then_increase_i t p 0 i';
+  = from_zero_to_i_bmh_does_not_return_i t p i;
+    bmh_not_equal_indices_then_increase_i t p 0 i';
     index_is_not_equal_belongs_false_base t p i'
 
-let boyer_moore_to_value_then_not_boyer_moore_to_length_p (t:list english_letters) (p:list english_letters{length p <= length t}) 
+let from_zero_to_i_belongs_is_false_implication (t:list english_letters) (p:list english_letters{length p <= length t}) 
+                                                (i:nat{i <= length t - length p}) (i':nat{i' < i})
+  : Lemma (ensures (forall (j:nat{j < i}). boyer_moore_horspool t p 0 j <> j) ==> belongs t p i' = false)
+  = move_requires (from_zero_to_i_belongs_is_false_base t p i) i'
+
+let from_zero_to_i_belongs_is_false (t:list english_letters) (p:list english_letters{length p <= length t}) 
+                                    (i:nat{i <= length t - length p})
+  : Lemma (ensures forall (i':nat{i' < i}). (forall (j:nat{j < i}). boyer_moore_horspool t p 0 j <> j) ==> belongs t p i' = false)
+  = forall_intro (from_zero_to_i_belongs_is_false_implication t p i)
+
+let bmh_to_value_then_not_bmh_to_length_p (t:list english_letters) (p:list english_letters{length p <= length t}) 
                                                           (k:nat{k < length p}) (i:nat{i <= length t - length p}) 
-  : Lemma (requires item_index (index t (i + length p - 1 - k)) alphabet 0 <> [] /\
-           last (item_index (index t (i + length p - 1 - k)) alphabet 0) < length (update_bc alphabet p) /\
+  : Lemma (requires item_indices (index t (i + length p - 1 - k)) alphabet 0 <> [] /\
+           last (item_indices (index t (i + length p - 1 - k)) alphabet 0) < length (update_bc alphabet p) /\
           (let bc = update_bc alphabet p in
-           let shiftbc = length p - k - 1 - index bc (last (item_index (index t (i + length p - 1 - k)) alphabet 0)) in
+           let shiftbc = length p - k - 1 - index bc (last (item_indices (index t (i + length p - 1 - k)) alphabet 0)) in
            let value = i + (maximum 1 shiftbc) in
-          //  boyer_moore t p 0 i = boyer_moore t p k i /\
            (forall (k':nat{k' < k}). index t (i + length p - 1 - k') = index p (length p - 1 - k')) /\
            index t (i + length p - 1 - k) <> index p (length p - 1 - k)))
-          (ensures boyer_moore t p k i <> boyer_moore t p (length p) i)
-  = assert(boyer_moore t p (length p) i = i);
+          (ensures boyer_moore_horspool t p k i <> boyer_moore_horspool t p (length p) i)
+  = assert(boyer_moore_horspool t p (length p) i = i);
     let bc = update_bc alphabet p in
-    let shiftbc = length p - k - 1 - index bc (last (item_index (index t (i + length p - 1 - k)) alphabet 0)) in
+    let shiftbc = length p - k - 1 - index bc (last (item_indices (index t (i + length p - 1 - k)) alphabet 0)) in
     let value = i + (maximum 1 shiftbc) in
     update_bc_length_is_initial_list_length alphabet p;
     assert(length bc = length alphabet);
-    boyer_moore_value_comparison t p 0 value
+    bmh_value_comparison t p 0 value
 
 let number_is_in_interval (i:nat) (i':nat{i' >= i && i' < i + 1})
   : Lemma (ensures i' = i)
   = ()
 
-let boyer_moore_belongs_false_if_less_than_shiftbc (t:list english_letters) (p:list english_letters{length p <= length t}) 
-                                                   (k:nat{k < length p}) (i:nat{i <= length t - length p}) 
-                                                   (i':nat{i' >= i})
-  : Lemma (requires item_index (index t (i + length p - 1 - k)) alphabet 0 <> [] /\
-           last (item_index (index t (i + length p - 1 - k)) alphabet 0) < length (update_bc alphabet p) /\
+#push-options "--split_queries always"
+let bmh_belongs_false_if_less_than_shiftbc (t:list english_letters) (p:list english_letters{length p <= length t}) 
+                                           (k:nat{k < length p}) (i:nat{i <= length t - length p}) 
+                                           (i':nat{i' >= i})
+  : Lemma (requires item_indices (index t (i + length p - 1 - k)) alphabet 0 <> [] /\
+           last (item_indices (index t (i + length p - 1 - k)) alphabet 0) < length (update_bc alphabet p) /\
           (let bc = update_bc alphabet p in
-           let shiftbc = length p - k - 1 - index bc (last (item_index (index t (i + length p - 1 - k)) alphabet 0)) in
+           let shiftbc = length p - k - 1 - index bc (last (item_indices (index t (i + length p - 1 - k)) alphabet 0)) in
            let value = i + (maximum 1 shiftbc) in
-           //boyer_moore t p 0 0 = boyer_moore t p 0 i /\ 
-           //boyer_moore t p 0 i = boyer_moore t p k i /\
            (forall (j:nat{j < i}). belongs t p j = false) /\
            (forall (k':nat{k' < k}). index t (i + length p - 1 - k') = index p (length p - 1 - k')) /\
            index t (i + length p - 1 - k) <> index p (length p - 1 - k) /\ i' < minimum value (length t - length p + 1)))
           (ensures belongs t p i' = false)
           (decreases length p - k)
   = let bc = update_bc alphabet p in
-    let shiftbc = length p - k - 1 - index bc (last (item_index (index t (i + length p - 1 - k)) alphabet 0)) in
+    let shiftbc = length p - k - 1 - index bc (last (item_indices (index t (i + length p - 1 - k)) alphabet 0)) in
     let value = i + (maximum 1 shiftbc) in
-    // assert(boyer_moore t p 0 0 = boyer_moore t p 0 i);
-    // assert(boyer_moore t p 0 i = boyer_moore t p k i);
     assert(forall (k':nat{k' < k}). index t (i + length p - 1 - k') = index p (length p - 1 - k'));
     assert(index t (i + length p - 1 - k) <> index p (length p - 1 - k));
-    item_index_of_t_in_alphabet t (i + length p - 1 - k);
-    last_is_less_than_bc t p (i + length p - 1 - k);
-    boyer_moore_to_value_then_not_boyer_moore_to_length_p t p k i;
-    assert(boyer_moore t p k i <> boyer_moore t p (length p) i);
-    //assert(boyer_moore t p k i = boyer_moore t p 0 value);
+    bmh_to_value_then_not_bmh_to_length_p t p k i;
+    assert(boyer_moore_horspool t p k i <> boyer_moore_horspool t p (length p) i);
+    assert(boyer_moore_horspool t p k i = boyer_moore_horspool t p 0 value);
     if shiftbc > 0
     then (
-      assert(index bc (last (item_index (index t (i + length p - 1 - k)) alphabet 0)) < length p - 1 - k);
+      assert(index bc (last (item_indices (index t (i + length p - 1 - k)) alphabet 0)) < length p - 1 - k);
       assert(i + length p - 1 - k >= 0 && i + length p - 1 - k < length t);
       update_bc_length_is_initial_list_length alphabet p;
-      update_bc_has_values_in_interval alphabet p (last (item_index (index t (i + length p - 1 - k)) alphabet 0));
-      assert(index bc (last (item_index (index t (i + length p - 1 - k)) alphabet 0)) = -1 || 
-            (index bc (last (item_index (index t (i + length p - 1 - k)) alphabet 0)) >= 0 &&
-              index bc (last (item_index (index t (i + length p - 1 - k)) alphabet 0)) < length p));
+      update_bc_has_values_in_interval alphabet p (last (item_indices (index t (i + length p - 1 - k)) alphabet 0));
+      assert(index bc (last (item_indices (index t (i + length p - 1 - k)) alphabet 0)) = -1 || 
+            (index bc (last (item_indices (index t (i + length p - 1 - k)) alphabet 0)) >= 0 &&
+              index bc (last (item_indices (index t (i + length p - 1 - k)) alphabet 0)) < length p));
 
-      let a = last (item_index (index t (i + length p - 1 - k)) alphabet 0) in 
-      let b = index bc (last (item_index (index t (i + length p - 1 - k)) alphabet 0)) in
+      let a = last (item_indices (index t (i + length p - 1 - k)) alphabet 0) in 
+      let b = index bc (last (item_indices (index t (i + length p - 1 - k)) alphabet 0)) in
         
       if b = -1 
       then (
-        update_bc_has_index_minusone_if_letter_is_not_in_pattern_forall_j alphabet p a;
+        update_bc_for_minusone_forall_j alphabet p a;
         assert(forall (j:nat{j < length p}). index p j <> index alphabet a);
 
-        mem_last_list (item_index (index t (i + length p - 1 - k)) alphabet 0);
-        assert(mem a (item_index (index t (i + length p - 1 - k)) alphabet 0) = true);
+        mem_last_list (item_indices (index t (i + length p - 1 - k)) alphabet 0);
+        assert(mem a (item_indices (index t (i + length p - 1 - k)) alphabet 0) = true);
           
         index_is_mem_is_item_base alphabet (index t (i + length p - 1 - k)) a;
         assert(index alphabet a = index t (i + length p - 1 - k));
         assert(forall (z:nat{z < length p}). index p z <> index t (i + length p - 1 - k))
       )
       else (
-        update_bc_has_correct_index_if_letter_is_in_pattern_base alphabet p a b;
+        update_bc_for_nat_base alphabet p a b;
         assert(index bc a = b);
         assert(index p b = index alphabet a);
         assert(forall (c:nat{c > b && c < length p}). index p c <> index alphabet a);
 
-        mem_last_list (item_index (index t (i + length p - 1 - k)) alphabet 0);
-        assert(mem a (item_index (index t (i + length p - 1 - k)) alphabet 0) = true);
+        mem_last_list (item_indices (index t (i + length p - 1 - k)) alphabet 0);
+        assert(mem a (item_indices (index t (i + length p - 1 - k)) alphabet 0) = true);
           
         index_is_mem_is_item_base alphabet (index t (i + length p - 1 - k)) a;
         assert(index alphabet a = index t (i + length p - 1 - k));
-        // assert(index p b = index t (i + length p - 1 - k));
         assert(forall (d:nat{d > b && d < length p}). index p d <> index t (i + length p - 1 - k));
 
         assert(shiftbc = maximum 1 shiftbc);
         assert(index t (i + length p - 1 - k) <> index p (length p - 1 - k));
           
-        // assert(b = index bc (last (item_index (index t (i + length p - 1 - k)) alphabet 0)));
-        // assert(b = length p - 1 - k - shiftbc);
-        // assert(index p (length p - 1 - k - shiftbc) = index t (i + length p - 1 - k));
         assert(value = i + shiftbc);
         assert(i' >= i && i' < i + shiftbc);
         assert(i' - i >= 0 && i' - i < shiftbc);
@@ -1124,43 +1085,39 @@ let boyer_moore_belongs_false_if_less_than_shiftbc (t:list english_letters) (p:l
       assert(minimum value (length t - length p + 1) = i + 1);
       assert(i' >= i && i' < i + 1);
       assert(i' = i);
-      assert(index t (i + length p - 1 - k) <> index p (length p - 1 - k))
+      assert(index t (i' + length p - 1 - k) <> index p (length p - 1 - k))
     );
     index_is_not_equal_belongs_false_base t p i';
     assert((exists (y:nat{y >= i' && y < i' + length p}). index t y <> index p (y - i')) ==> belongs t p i' = false);
     assert(i + length p - 1 - k >= i')
-    // assert(i + length p - 1 - k < i' + length p)
+#pop-options
 
-let boyer_moore_belongs_false_if_less_than_shiftbc_implication (t:list english_letters) (p:list english_letters{length p <= length t}) 
+let bmh_belongs_false_if_less_than_shiftbc_implication (t:list english_letters) (p:list english_letters{length p <= length t}) 
                                                                (k:nat{k < length p}) (i:nat{i <= length t - length p}) 
                                                                (i':nat{i' >= i})
-  : Lemma (ensures (item_index (index t (i + length p - 1 - k)) alphabet 0 <> [] /\
-           last (item_index (index t (i + length p - 1 - k)) alphabet 0) < length (update_bc alphabet p) /\
+  : Lemma (ensures (item_indices (index t (i + length p - 1 - k)) alphabet 0 <> [] /\
+           last (item_indices (index t (i + length p - 1 - k)) alphabet 0) < length (update_bc alphabet p) /\
           (let bc = update_bc alphabet p in
-           let shiftbc = length p - k - 1 - index bc (last (item_index (index t (i + length p - 1 - k)) alphabet 0)) in
+           let shiftbc = length p - k - 1 - index bc (last (item_indices (index t (i + length p - 1 - k)) alphabet 0)) in
            let value = i + (maximum 1 shiftbc) in
-          //  boyer_moore t p 0 0 = boyer_moore t p 0 i /\ 
-          //  boyer_moore t p 0 i = boyer_moore t p k i /\
            (forall (j:nat{j < i}). belongs t p j = false) /\
            (forall (k':nat{k' < k}). index t (i + length p - 1 - k') = index p (length p - 1 - k')) /\
            index t (i + length p - 1 - k) <> index p (length p - 1 - k) /\ i' < minimum value (length t - length p + 1)))
            ==> belongs t p i' = false)
-  = move_requires (boyer_moore_belongs_false_if_less_than_shiftbc t p k i) i'
+  = move_requires (bmh_belongs_false_if_less_than_shiftbc t p k i) i'
 
-let boyer_moore_belongs_false_if_less_than_shiftbc_forall (t:list english_letters) (p:list english_letters{length p <= length t}) 
+let bmh_belongs_false_if_less_than_shiftbc_forall (t:list english_letters) (p:list english_letters{length p <= length t}) 
                                                           (k:nat{k < length p}) (i:nat{i <= length t - length p}) 
-  : Lemma (ensures forall (i':nat{i' >= i}). (item_index (index t (i + length p - 1 - k)) alphabet 0 <> [] /\
-           last (item_index (index t (i + length p - 1 - k)) alphabet 0) < length (update_bc alphabet p) /\
+  : Lemma (ensures forall (i':nat{i' >= i}). (item_indices (index t (i + length p - 1 - k)) alphabet 0 <> [] /\
+           last (item_indices (index t (i + length p - 1 - k)) alphabet 0) < length (update_bc alphabet p) /\
           (let bc = update_bc alphabet p in
-           let shiftbc = length p - k - 1 - index bc (last (item_index (index t (i + length p - 1 - k)) alphabet 0)) in
+           let shiftbc = length p - k - 1 - index bc (last (item_indices (index t (i + length p - 1 - k)) alphabet 0)) in
            let value = i + (maximum 1 shiftbc) in
-          //  boyer_moore t p 0 0 = boyer_moore t p 0 i /\ 
-          //  boyer_moore t p 0 i = boyer_moore t p k i /\
            (forall (j:nat{j < i}). belongs t p j = false) /\
            (forall (k':nat{k' < k}). index t (i + length p - 1 - k') = index p (length p - 1 - k')) /\
            index t (i + length p - 1 - k) <> index p (length p - 1 - k) /\ i' < minimum value (length t - length p + 1)))
            ==> belongs t p i' = false)
-  = forall_intro (boyer_moore_belongs_false_if_less_than_shiftbc_implication t p k i)
+  = forall_intro (bmh_belongs_false_if_less_than_shiftbc_implication t p k i)
 
 let forall_true_and_for_k_true_then_forall_plus_one_true (t:list english_letters) (p:list english_letters{length p <= length t})
                                                          (k:nat{k < length p}) (i:nat{i <= length t - length p})
@@ -1169,96 +1126,100 @@ let forall_true_and_for_k_true_then_forall_plus_one_true (t:list english_letters
           (ensures forall (k':nat{k' < k + 1}). index t (i + length p - 1 - k') = index p (length p - 1 - k'))
   = ()
 
-let rec boyer_moore_gives_correct_result (t:list english_letters) (p:list english_letters{length p <= length t})
+let rec bmh_gives_correct_result (t:list english_letters) (p:list english_letters{length p <= length t})
                                          (k:nat{k <= length p}) (i:nat{i <= length t - length p})
-  : Lemma (requires //boyer_moore t p 0 0 = boyer_moore t p 0 i /\ 
+  : Lemma (requires  
            (forall (i':nat{i' < i}). belongs t p i' = false) /\ 
-          //  boyer_moore t p 0 i = boyer_moore t p k i /\
            (forall (k':nat{k' < k}). index t (i + length p - 1 - k') = index p (length p - 1 - k')))
           (ensures 
-          (let x = boyer_moore t p k i in 
+          (let x = boyer_moore_horspool t p k i in 
            x <> -1 ==> belongs t p x = true))
           (decreases %[(if i < length t - length p + 1 then length t - length p + 1 - i else 0); length p - k])
-  = if k = length p
+  = let m = length p in
+    if k = m
     then (
-      assert(forall (k':nat{k' < length p}). index t (i + length p - 1 - k') = index p (length p - 1 - k'));
+      assert(forall (k':nat{k' < m}). index t (i + m - 1 - k') = index p (m - 1 - k'));
       indices_are_equal_belongs_true_base t p i;
       convert_from_x_to_j p i
     )
     else (
-      if index t (i + length p - 1 - k) = index p (length p - 1 - k)
+      if index t (i + m - 1 - k) = index p (m - 1 - k)
       then (
-        zero_to_k_than_all_indices_are_equal t p k i;
-        boyer_moore_gives_correct_result t p (k + 1) i 
+        zero_to_k_then_all_indices_are_equal t p k i;
+        bmh_gives_correct_result t p (k + 1) i 
       )
       else (
-        item_index_of_t_in_alphabet t (i + length p - 1 - k);
-        last_is_less_than_bc t p (i + length p - 1 - k);
-        let shiftbc = length p - k - 1 - index (update_bc alphabet p) (last (item_index (index t (i + length p - 1 - k)) alphabet 0)) in
+        update_bc_length_is_initial_list_length alphabet p;
+        mem_last_list (item_indices (index t (i + m - 1 - k)) alphabet 0);
+        item_indices_is_in_interval_forall alphabet 0 (index t (i + m - 1 - k));
+        let shiftbc = m - k - 1 - index (update_bc alphabet p) (last (item_indices (index t (i + m - 1 - k)) alphabet 0)) in
         let value = i + (maximum 1 shiftbc) in
-        if value > length t - length p
+        if value > length t - m
         then ()
         else (
-          boyer_moore_belongs_false_if_less_than_shiftbc_forall t p k i;
-          boyer_moore_gives_correct_result t p 0 value
+          bmh_belongs_false_if_less_than_shiftbc_forall t p k i;
+          bmh_gives_correct_result t p 0 value
         )
       )
     )
 
-let boyer_moore_gives_correct_result_for_text_and_pattern ()
+let bmh_gives_correct_result_for_text_and_pattern ()
   : Lemma (ensures 
-          (let x = boyer_moore text pattern 0 0 in 
+          (let x = boyer_moore_horspool text pattern 0 0 in 
            x <> -1 ==> belongs text pattern x = true))
   = assert(0 <= length text - length pattern);
-    boyer_moore_gives_correct_result text pattern 0 0
+    bmh_gives_correct_result text pattern 0 0
 
-//for requires 
-let rec boyer_moore_gives_minus_one_belongs_false (t:list english_letters) (p:list english_letters{length p <= length t})
+let rec bmh_gives_minus_one_belongs_false (t:list english_letters) (p:list english_letters{length p <= length t})
                                                   (k:nat{k <= length p}) (i:nat{i <= length t - length p})
-  : Lemma (requires //boyer_moore t p 0 0 = boyer_moore t p 0 i /\ 
+  : Lemma (requires  
            (forall (i':nat{i' < i}). belongs t p i' = false) /\ 
-          //  boyer_moore t p 0 i = boyer_moore t p k i /\
            (forall (k':nat{k' < k}). index t (i + length p - 1 - k') = index p (length p - 1 - k')))
           (ensures 
-          (let x = boyer_moore t p k i in 
+          (let x = boyer_moore_horspool t p k i in 
            x = -1 ==> (forall (y:nat{y <= length t - length p}). belongs t p y = false)))
           (decreases %[(if i < length t - length p + 1 then length t - length p + 1 - i else 0); length p - k])
-  = if k = length p 
+  = let m = length p in
+    if k = m 
     then ()
     else (
-      assert(k < length p);
-      if index t (i + length p - 1 - k) = index p (length p - 1 - k)
+      assert(k < m);
+      if index t (i + m - 1 - k) = index p (m - 1 - k)
       then (
-        zero_to_k_than_all_indices_are_equal t p k i;
-        boyer_moore_gives_minus_one_belongs_false t p (k + 1) i
+        zero_to_k_then_all_indices_are_equal t p k i;
+        bmh_gives_minus_one_belongs_false t p (k + 1) i
       )
       else (
-        item_index_of_t_in_alphabet t (i + length p - 1 - k);
-        last_is_less_than_bc t p (i + length p - 1 - k);
-        let shiftbc = length p - k - 1 - index (update_bc alphabet p) (last (item_index (index t (i + length p - 1 - k)) alphabet 0)) in
+        update_bc_length_is_initial_list_length alphabet p;
+        mem_last_list (item_indices (index t (i + m - 1 - k)) alphabet 0);
+        item_indices_is_in_interval_forall alphabet 0 (index t (i + m - 1 - k));
+        let shiftbc = m - k - 1 - index (update_bc alphabet p) (last (item_indices (index t (i + m - 1 - k)) alphabet 0)) in
         let value = i + (maximum 1 shiftbc) in
-        boyer_moore_belongs_false_if_less_than_shiftbc_forall t p k i; 
-        if value > length t - length p 
+        bmh_belongs_false_if_less_than_shiftbc_forall t p k i; 
+        if value > length t - m
         then ()
-        else boyer_moore_gives_minus_one_belongs_false t p 0 value
+        else bmh_gives_minus_one_belongs_false t p 0 value
       )
     )
 
-let boyer_moore_gives_minus_one_belongs_false_for_text_and_pattern ()
+let bmh_gives_minus_one_belongs_false_for_text_and_pattern ()
   : Lemma (ensures 
-          (let x = boyer_moore text pattern 0 0 in 
+          (let x = boyer_moore_horspool text pattern 0 0 in 
            x = -1 ==> (forall (y:nat{y <= length text - length pattern}). belongs text pattern y = false)))
-  = boyer_moore_gives_minus_one_belongs_false text pattern 0 0
+  = bmh_gives_minus_one_belongs_false text pattern 0 0
 
-let string_of_int_list l =
-Printf.sprintf "[%s]"
-(String.concat "; " (List.Tot.map (Printf.sprintf "%d") l))
+//output verification
+let rec convert_english_letters_to_int (l:list english_letters)
+  : list int 
+  = match l with 
+    | [] -> []
+    | hd :: tl -> if hd = A then 
+                  0 :: convert_english_letters_to_int tl 
+                  else 1 :: convert_english_letters_to_int tl
 
 let main() =
   let message =
-     if length pattern <= length text
-     then sprintf "The result is %d." (boyer_moore text pattern 0 0)
-     else sprintf "The length of the pattern needs to be less or equal to the length of the text!"
+     sprintf "The result is %d." (boyer_moore_horspool text pattern 0 0)
   in
   print_string message
 
