Belongs.fst
@@ -1,0 +1,100 @@
+module Belongs
+
+open UpdateBc
+open GlobalData
+open ItemIndices
+open NewOrOld
+open FStar.Classical 
+open FStar.IO
+open FStar.Printf
+open FStar.List
+open FStar.List.Tot.Base
+
+let rec belongs (t:list english_letters) (p:list english_letters{length p <= length t}) (i:nat)
+  : bool 
+  = match p with
+    | [] -> true
+    | hd :: tl -> if i < length t && hd = index t i 
+                  then belongs t tl (i + 1)
+                  else false
+
+let rec belongs_true_index_is_equal_base (t:list english_letters) (p:list english_letters{length p <= length t}) (i:nat{i <= length t - length p}) (j:nat{j >= i && j < i + length p})
+  : Lemma (ensures belongs t p i = true ==> index t j = index p (j - i))
+  = match p with 
+    | [] -> ()
+    | hd :: tl -> if hd = index t i 
+                  then (
+                    assert(belongs t p i = belongs t tl (i + 1));
+                    if i < j 
+                    then belongs_true_index_is_equal_base t tl (i + 1) j
+                    else ()
+                  )
+                  else ()
+
+let belongs_true_indices_are_equal (t:list english_letters) (p:list english_letters{length p <= length t})
+  : Lemma (ensures forall (i:nat{i <= length t - length p}) (j:nat{j >= i && j < i + length p}). belongs t p i = true ==> index t j = index p (j - i))
+  = forall_intro_2 (belongs_true_index_is_equal_base t p)
+
+let rec belongs_false_index_is_not_equal_base (t:list english_letters) (p:list english_letters{length p <= length t}) (i:nat{i <= length t - length p}) 
+  : Lemma (ensures belongs t p i = false ==> (exists (j:nat{j >= i && j < i + length p}). index t j <> index p (j - i)))
+  = match p with 
+    | [] -> ()
+    | hd :: tl -> if hd = index t i 
+                  then belongs_false_index_is_not_equal_base t tl (i + 1)
+                  else ()
+
+let belongs_false_index_is_not_equal (t:list english_letters) (p:list english_letters{length p <= length t})
+  : Lemma (ensures forall (i:nat{i <= length t - length p}) . belongs t p i = false ==> (exists (j:nat{j >= i && j < i + length p}). index t j <> index p (j - i)))
+  = forall_intro (belongs_false_index_is_not_equal_base t p)
+
+let rec index_is_not_equal_belongs_false_base (t:list english_letters) (p:list english_letters{length p <= length t}) (i:nat{i <= length t - length p})
+  : Lemma (ensures (exists (j:nat{j >= i && j < i + length p}). index t j <> index p (j - i)) ==> belongs t p i = false)
+  = match p with 
+    | [] -> ()
+    | hd :: tl -> if hd <> index t i
+                  then ()
+                  else index_is_not_equal_belongs_false_base t tl (i + 1)
+
+let index_is_not_equal_belongs_false (t:list english_letters) (p:list english_letters{length p <= length t}) 
+  : Lemma (ensures forall (i:nat{i <= length t - length p}). (exists (j:nat{j >= i && j < i + length p}). index t j <> index p (j - i)) ==> belongs t p i = false)
+  = forall_intro (index_is_not_equal_belongs_false_base t p)
+
+let rec indices_are_equal_belongs_true_base (t:list english_letters) (p:list english_letters{length p <= length t}) (i:nat{i <= length t - length p})
+  : Lemma (ensures (forall (j:nat{j >= i && j < i + length p}). index t j = index p (j - i)) ==> belongs t p i = true)
+  = match p with 
+    | [] -> ()
+    | hd :: tl -> if hd <> index t i 
+                  then ()
+                  else indices_are_equal_belongs_true_base t tl (i + 1)
+
+let indices_are_equal_belongs_true (t:list english_letters) (p:list english_letters{length p <= length t})
+  : Lemma (ensures forall (i:nat{i <= length t - length p}). (forall (j:nat{j >= i && j < i + length p}). index t j = index p (j - i)) ==> belongs t p i = true)
+  = forall_intro (indices_are_equal_belongs_true_base t p)
+
+let maximum (a:int) (b:int)
+  : int 
+  = if a > b 
+    then a 
+    else b 
+
+let maximum_returns_correct_result_base (a:int) (b:int)
+  : Lemma (ensures maximum a b = a ==> a >= b)
+  = ()
+
+let maximum_returns_correct_result ()
+  : Lemma (ensures forall (a:int) (b:int). maximum a b = a ==> a >= b)
+  = forall_intro_2 maximum_returns_correct_result_base
+
+let minimum (a:int) (b:int)
+  : int 
+  = if a > b 
+    then b 
+    else a 
+
+let minimum_returns_correct_result_base (a:int) (b:int)
+  : Lemma (ensures minimum a b = a ==> a <= b)
+  = ()
+
+let minimum_returns_correct_result ()
+  : Lemma (ensures forall (a:int) (b:int). minimum a b = a ==> a <= b)
+  = forall_intro_2 minimum_returns_correct_result_base
