GlobalData.fst
@@ -1,0 +1,52 @@
+module GlobalData
+
+open FStar.Classical 
+open FStar.IO
+open FStar.Printf
+open FStar.List
+open FStar.List.Tot.Base
+
+type english_letters =
+  | A
+  | B
+
+val alphabet : (l:list english_letters{(forall (x:english_letters). mem x l = true) /\ l <> []})
+let alphabet = [A;B]
+  
+val text : (l:list english_letters{l <> []})
+let text = [A;A;A;A;B;A;A;B;A;B;A;A;A;B;A;B;B]
+
+let rec l1_length_less_than_l2_length (l1:list english_letters) (l2:list english_letters)
+  : bool
+  = if length l1 > 0 && length l2 > 0 
+    then l1_length_less_than_l2_length (tail l1) (tail l2)
+    else (
+      if length l1 = 0 
+      then true
+      else false
+    )
+
+let rec l1_less_true (l1:list english_letters) (l2:list english_letters)
+  : Lemma (requires l1_length_less_than_l2_length l1 l2 = true)
+          (ensures length l1 <= length l2)
+  = if length l1 > 0 && length l2 > 0 
+    then l1_less_true (tail l1) (tail l2)
+    else ()
+
+let rec l1_less_false (l1:list english_letters) (l2:list english_letters)
+  : Lemma (requires l1_length_less_than_l2_length l1 l2 = false)
+          (ensures length l1 > length l2)
+  = if length l1 > 0 && length l2 > 0 
+    then l1_less_false (tail l1) (tail l2)
+    else ()
+
+let candidate : list english_letters 
+  = [A;A;B;A;A;A;B;A;B]
+
+val pattern : (l:list english_letters{length l <= length text})
+let pattern = if l1_length_less_than_l2_length candidate text = true
+              then (
+                l1_less_true candidate text;
+                candidate
+              )
+              else []
