ItemIndices.fst
@@ -1,0 +1,367 @@
+module ItemIndices
+
+open GlobalData
+open FStar.Classical 
+open FStar.IO
+open FStar.Printf
+open FStar.List
+open FStar.List.Tot.Base
+
+let rec item_indices (#a:eqtype) (item:a) (l:list a) (i:nat) 
+  : list nat
+  = match l with 
+    | [] -> []
+    | hd :: tl -> if hd = item
+                  then i :: item_indices item tl (i + 1)
+                  else item_indices item tl (i + 1)
+
+let rec item_list_has_correct_length (#a:eqtype) (l:list a) (i:nat)
+  : Lemma (ensures forall (item:a). length (item_indices item l i) = count item l)
+  = match l with 
+    | [] -> ()
+    | hd :: tl -> item_list_has_correct_length tl (i + 1)
+
+let rec item_indices_is_in_interval (#a:eqtype) (item:a) (l:list a) (i:nat) (x:nat)
+  : Lemma (ensures mem x (item_indices item l i) ==> i <= x && x < i + length l)
+  = match l with 
+    | [] -> () 
+    | hd :: tl -> item_indices_is_in_interval item tl (i + 1) x 
+
+let item_indices_is_in_interval_forall (#a:eqtype) (l:list a) (i:nat) (item:a)
+  : Lemma (ensures forall (x:nat). mem x (item_indices item l i) ==> i <= x && x < i + length l)
+  = forall_intro (item_indices_is_in_interval item l i)
+
+let item_indices_is_in_interval_forall_item (#a:eqtype) (l:list a) (i:nat)
+  : Lemma (ensures forall (item:a) (x:nat). mem x (item_indices item l i) ==> i <= x && x < i + length l)
+  = forall_intro (item_indices_is_in_interval_forall l i)
+
+let rec item_indices_one_and_item_indices_zero (#a:eqtype) (item:a) (l:list a) (x:nat{x > 0}) (i:nat{i > 0})
+  : Lemma (ensures mem x (item_indices item l i) = mem (x - 1) (item_indices item l (i - 1)))
+  = match l with 
+    | [] -> ()
+    | hd :: tl -> match x with 
+                  | 1 -> if i = 1
+                         then (
+                          if hd = item 
+                          then ()
+                          else (
+                           item_indices_is_in_interval item tl (i + 1) x;
+                           item_indices_is_in_interval item tl i (x - 1)
+                          )
+                         )
+                         else (
+                           item_indices_is_in_interval item l i x;
+                           item_indices_is_in_interval item l (i - 1) (x - 1)
+                         )
+                  | _ -> if i > x
+                         then (
+                          item_indices_is_in_interval item l i x;
+                          item_indices_is_in_interval item l (i - 1) (x - 1)
+                         )
+                         else (
+                          if i = x 
+                          then (
+                            if hd = item 
+                            then ()
+                            else (
+                             item_indices_is_in_interval item tl (i + 1) x;
+                             item_indices_is_in_interval item tl i (x - 1)
+                            )
+                          )
+                          else (
+                            assert(mem x (item_indices item l i) = mem x (item_indices item tl (i + 1)));
+                            assert(mem (x - 1) (item_indices item l (i - 1)) = mem (x - 1) (item_indices item tl i));
+                            item_indices_one_and_item_indices_zero item tl x (i + 1)
+                          )
+                         )
+
+let rec index_increases_with_one_when_element_is_added (#a:eqtype) (item:a) (l:list a) (i:nat{i > 0}) (el:a)
+  : Lemma (ensures mem (i - 1) (item_indices item l 0) = false ==> mem i (item_indices item (el :: l) 0) = false)
+  = match l with 
+    | [] -> ()
+    | hd :: tl -> match i with 
+                  | 1 -> if hd = item 
+                         then ()
+                         else item_indices_is_in_interval item tl 2 1
+                  | _ -> item_indices_one_and_item_indices_zero item l i 1;
+                         index_increases_with_one_when_element_is_added item tl (i - 1) hd
+
+let rec index_increases_with_one_when_element_is_added_for_true (#a:eqtype) (item:a) (l:list a) (i:nat{i > 0}) (el:a)
+  : Lemma (ensures mem (i - 1) (item_indices item l 0) = true ==> mem i (item_indices item (el :: l) 0) = true)
+  = match l with 
+    | [] -> ()
+    | hd :: tl -> match i with 
+                  | 1 -> if hd = item 
+                         then ()
+                         else item_indices_is_in_interval item tl i (i - 1)
+                  | _ -> item_indices_one_and_item_indices_zero item l i 1;
+                         index_increases_with_one_when_element_is_added_for_true item tl (i - 1) hd
+
+let rec index_increases_with_one_when_first_is_item (#a:eqtype) (item:a) (l:list a) (i:nat{i > 0})
+  : Lemma (ensures mem (i - 1) (item_indices item l 0) = false ==> mem i (0 :: item_indices item l 1) = false)
+  = match l with 
+    | [] -> ()
+    | hd :: tl -> match i with 
+                  | 1 -> if hd = item 
+                         then ()
+                         else item_indices_is_in_interval item tl 2 1
+                  | _ -> item_indices_one_and_item_indices_zero item l i 1;
+                         index_increases_with_one_when_first_is_item item tl (i - 1)
+
+let rec index_increases_with_one_when_first_is_item_for_true (#a:eqtype) (item:a) (l:list a) (i:nat{i > 0})
+  : Lemma (ensures mem (i - 1) (item_indices item l 0) = true ==> mem i (0 :: item_indices item l 1) = true)
+  = match l with 
+    | [] -> ()
+    | hd :: tl -> match i with 
+                  | 1 -> if hd = item 
+                         then ()
+                         else item_indices_is_in_interval item tl i (i - 1)
+                  | _ -> item_indices_one_and_item_indices_zero item l i 1;
+                         index_increases_with_one_when_first_is_item_for_true item tl (i - 1)
+
+let rec index_is_not_item_is_not_mem_base (#a:eqtype) (l:list a) (item:a) (i:nat{i < length l})
+  : Lemma (ensures index l i <> item ==> mem i (item_indices item l 0) = false)
+  = match l with
+    | [] -> ()
+    | hd :: tl -> match i with 
+                  | 0 -> if hd = item 
+                         then ()
+                         else item_indices_is_in_interval item tl (i + 1) i
+                  | _ -> if hd = item 
+                         then index_increases_with_one_when_first_is_item item tl i
+                         else index_increases_with_one_when_element_is_added item tl i hd;
+                         index_is_not_item_is_not_mem_base tl item (i - 1)
+
+let index_is_not_item_is_not_mem (#a:eqtype) (l:list a) 
+  : Lemma (ensures forall (item:a) (i:nat{i < length l}). index l i <> item ==> mem i (item_indices item l 0) = false)
+  = forall_intro_2 (index_is_not_item_is_not_mem_base l)
+
+let rec index_is_item_is_mem_base (#a:eqtype) (l:list a) (item:a) (i:nat{i < length l})
+  : Lemma (ensures index l i = item ==> mem i (item_indices item l 0) = true)
+  = match l with
+    | [] -> ()
+    | hd :: tl -> match i with 
+                  | 0 -> if hd = item
+                         then ()
+                         else item_indices_is_in_interval item tl (i + 1) i
+                  | _ -> assert(index l i = index tl (i - 1));
+                         if hd = item
+                         then index_increases_with_one_when_first_is_item_for_true item tl i 
+                         else index_increases_with_one_when_element_is_added_for_true item tl i hd;
+                         index_is_item_is_mem_base tl item (i - 1)
+
+let index_is_item_is_mem (#a:eqtype) (l:list a)
+  : Lemma (ensures forall (item:a) (i:nat{i < length l}). index l i = item ==> mem i (item_indices item l 0) = true)
+  = forall_intro_2 (index_is_item_is_mem_base l)
+
+let rec index_is_not_mem_is_not_item_base (#a:eqtype) (l:list a) (item:a) (i:nat{i < length l})
+  : Lemma (ensures mem i (item_indices item l 0) = false ==> index l i <> item)
+  = match l with
+    | [] -> ()
+    | hd :: tl -> match i with 
+                  | 0 -> if hd = item 
+                         then ()
+                         else item_indices_is_in_interval item tl (i + 1) i
+                  | _ -> index_is_not_mem_is_not_item_base tl item (i - 1);
+                         item_indices_one_and_item_indices_zero item tl i 1
+
+let index_is_not_mem_is_not_item_forall_i (#a:eqtype) (l:list a) (item:a)
+  : Lemma (ensures forall (i:nat{i < length l}). mem i (item_indices item l 0) = false ==> index l i <> item)
+  = forall_intro (index_is_not_mem_is_not_item_base l item)
+
+let index_is_not_mem_is_not_item (#a:eqtype) (l:list a)
+  : Lemma (ensures forall (item:a) (i:nat{i < length l}). mem i (item_indices item l 0) = false ==> index l i <> item)
+  = forall_intro (index_is_not_mem_is_not_item_forall_i l)
+
+let rec index_is_mem_is_item_base (#a:eqtype) (l:list a) (item:a) (i:nat{i < length l})
+  : Lemma (ensures mem i (item_indices item l 0) = true ==> index l i = item)
+  = match l with
+    | [] -> ()
+    | hd :: tl -> match i with 
+                  | 0 -> if hd = item 
+                         then ()
+                         else item_indices_is_in_interval item tl (i + 1) i
+                  | _ -> index_is_mem_is_item_base tl item (i - 1);
+                         item_indices_one_and_item_indices_zero item tl i 1
+
+let index_is_mem_is_item_forall_i (#a:eqtype) (l:list a) (item:a)
+  : Lemma (ensures forall (i:nat{i < length l}). mem i (item_indices item l 0) = true ==> index l i = item)
+  = forall_intro (index_is_mem_is_item_base l item)
+
+let index_is_mem_is_item (#a:eqtype) (l:list a)
+  : Lemma (ensures forall (item:a) (i:nat{i < length l}). mem i (item_indices item l 0) = true ==> index l i = item)
+  = forall_intro (index_is_mem_is_item_forall_i l)
+
+let index_not_mem_not_item_not_item_not_mem (#a:eqtype) (l:list a)
+  : Lemma (ensures forall (item:a) (i:nat{i < length l}). mem i (item_indices item l 0) = false <==> index l i <> item)
+  = index_is_not_item_is_not_mem l;
+    index_is_not_mem_is_not_item l
+
+let index_mem_item_item_mem (#a:eqtype) (l:list a)
+  : Lemma (ensures forall (item:a) (i:nat{i < length l}). mem i (item_indices item l 0) = true <==> index l i = item)
+  = index_is_mem_is_item l;
+    index_is_item_is_mem l
+
+let rec mem_index_element (#a:eqtype) (l:list a) (i:nat{i < length l})
+  : Lemma (ensures mem (index l i) l = true)
+  = match l with 
+    | [] -> ()
+    | hd :: tl -> match i with
+                  | 0 -> ()
+                  | _ -> mem_index_element tl (i - 1)
+
+let mem_index_element_forall (#a:eqtype) (l:list a)
+  : Lemma (ensures forall (i:nat{i < length l}). mem (index l i) l = true)
+  = forall_intro (mem_index_element l)
+
+let rec index_not_zero_not_first_element (#a:eqtype) (l:list a) (item:a) (m:nat) (i:nat{i < length (item_indices item l m)})
+  : Lemma (requires length (item_indices item l m) > 1)
+          (ensures 
+           (let indices = item_indices item l m in
+            i <> 0 ==> index indices i <> hd indices))
+  = match l with 
+    | [] -> ()
+    | fst :: tl -> if fst = item 
+                   then (
+                    assert(hd (item_indices item l m) = m);
+                    assert(item_indices item l m = m :: (item_indices item tl (m + 1)));
+                    match i with 
+                    | 0 -> ()
+                    | _ -> mem_index_element (item_indices item tl (m + 1)) (i - 1);
+                           item_indices_is_in_interval item tl (m + 1) (index (item_indices item tl (m + 1)) (i - 1))
+                   )
+                   else index_not_zero_not_first_element tl item (m + 1) i
+
+let rec hd_item_indices_is_min (#a:eqtype) (l:list a) (item:a) (i:nat) (m:nat)
+  : Lemma (requires length (item_indices item l m) > 1)
+          (ensures 
+           (let indices = item_indices item l m in 
+            mem i indices && i <> hd indices ==> i > hd indices))
+  = match l with 
+    | [] -> ()
+    | fst :: tl -> if fst = item 
+                   then item_indices_is_in_interval item tl (m + 1) i
+                   else hd_item_indices_is_min tl item i (m + 1)
+
+let subtraction (i:nat) : nat
+  = if i > 0
+    then i - 1
+    else i
+
+let proof_subtraction (i:nat)
+  : Lemma (ensures i > 0 ==> subtraction i = i - 1)
+  = ()
+
+let rec item_indices_zero_is_item_indices_one_minus_one (#a:eqtype) (l:list a) (item:a) (m:nat)
+  : Lemma (ensures item_indices item l m = map subtraction (item_indices item l (m + 1)))
+  = match l with 
+    | [] -> ()
+    | hd :: tl -> item_indices_zero_is_item_indices_one_minus_one tl item (m + 1)
+
+let rec item_map_subtraction (l:list nat) (i:nat{i < length l})
+  : Lemma (ensures 
+           (let l' = map subtraction l in
+            index l i > 0 ==> index l' i = (index l i) - 1))
+  = match l with
+    | [] -> ()
+    | fst :: tl -> match i with 
+                  | 0 -> ()
+                  | _ -> item_map_subtraction tl (i - 1)
+
+let rec indices_are_ordered_in_ascending_order_base (#a:eqtype) (l:list a) (item:a) 
+        (i:nat{i < length (item_indices item l 0)}) (j:nat{j < length (item_indices item l 0)})
+  : Lemma (requires i < j)
+          (ensures 
+           (let indices = item_indices item l 0 in
+            index indices i < index indices j))
+  = match l with 
+    | [] -> ()
+    | fst :: tl -> let l' = item_indices item l 0 in 
+                   let l'' = item_indices item tl 1 in
+                   let l''' = item_indices item tl 0 in
+                   match i with 
+                  | 0 -> if fst = item 
+                         then (
+                          mem_index_element l'' (j - 1);
+                          item_indices_is_in_interval item tl 1 (index l'' (j - 1))
+                         )
+                         else (
+                          if length l'' < 2
+                          then ()
+                          else (
+                            mem_index_element l' j;
+                            index_not_zero_not_first_element l item 0 j;
+                            hd_item_indices_is_min l item (index l' j) 0
+                          )
+                         )
+                  | _ -> item_indices_zero_is_item_indices_one_minus_one tl item 0;
+                         assert(l''' = map subtraction l'');
+                         if fst = item
+                         then (
+                          assert(index l' i = index l'' (i - 1));
+                          assert(index l' j = index l'' (j - 1));
+                          mem_index_element l'' (i - 1);
+                          mem_index_element l'' (j - 1);
+                          item_map_subtraction l'' (i - 1);
+                          item_map_subtraction l'' (j - 1);
+                          item_indices_is_in_interval item tl 1 (index l'' (i - 1));
+                          item_indices_is_in_interval item tl 1 (index l'' (j - 1));
+                          assert(index l''' (i - 1) = (index l'' (i - 1)) - 1);
+                          assert(index l''' (j - 1) = (index l'' (j - 1)) - 1);
+                          indices_are_ordered_in_ascending_order_base tl item (i - 1) (j - 1)
+                         )
+                         else (
+                          assert(index l' i = index l'' i);
+                          assert(index l' j = index l'' j);
+                          mem_index_element l'' i;
+                          mem_index_element l'' j;
+                          item_map_subtraction l'' i;
+                          item_map_subtraction l'' j;
+                          item_indices_is_in_interval item tl 1 (index l'' i);
+                          item_indices_is_in_interval item tl 1 (index l'' j);
+                          assert(index l''' i = (index l'' i) - 1);
+                          assert(index l''' j = (index l'' j) - 1);
+                          indices_are_ordered_in_ascending_order_base tl item i j 
+                         )
+
+let indices_are_ordered_in_ascending_order_implication (#a:eqtype) (l:list a) (item:a)
+  (i:nat{i < length (item_indices item l 0)}) (j:nat{j < length (item_indices item l 0)})
+  : Lemma (ensures i < j ==>
+           (let indices = item_indices item l 0 in
+            index indices i < index indices j))
+  = move_requires (indices_are_ordered_in_ascending_order_base l item i) j
+
+let indices_are_ordered_in_ascending_order (#a:eqtype) (l:list a) (item:a)
+  : Lemma (ensures forall (i:nat{i < length (item_indices item l 0)}) (j:nat{j < length (item_indices item l 0)}). 
+           i < j ==>
+           (let indices = item_indices item l 0 in
+            index indices i < index indices j))
+  = forall_intro_2 (indices_are_ordered_in_ascending_order_implication l item)
+
+let indices_are_ordered_in_ascending_order_forall_item (#a:eqtype) (l:list a)
+  : Lemma (ensures forall (item:a) (i:nat{i < length (item_indices item l 0)}) (j:nat{j < length (item_indices item l 0)}). 
+           i < j ==>
+           (let indices = item_indices item l 0 in
+            index indices i < index indices j))
+  = forall_intro (indices_are_ordered_in_ascending_order l)
+
+let rec last_is_length_l_minus_one (#a:eqtype) (l:list a)
+  : Lemma (requires l <> [])
+          (ensures last l = index l ((length l) - 1))
+  = match l with
+    | [el] -> ()
+    | hd :: tl -> last_is_length_l_minus_one tl
+
+let last_index_is_max_base (#a:eqtype) (item:a) (l:list a{item_indices item l 0 <> []}) (i:nat{i < length (item_indices item l 0) - 1})
+  : Lemma (ensures 
+           (let indices = item_indices item l 0 in
+            let j = (length indices) - 1 in
+            index indices i < index indices j))
+  = indices_are_ordered_in_ascending_order_base l item i (length (item_indices item l 0) - 1)
+
+let last_index_is_max (#a:eqtype) (item:a) (l:list a{item_indices item l 0 <> []}) 
+  : Lemma (ensures forall (i:nat{i < length (item_indices item l 0) - 1}).
+           (let indices = item_indices item l 0 in
+            let j = (length indices) - 1 in
+            index indices i < index indices j))
+  = forall_intro (last_index_is_max_base item l)
