Main.fst
@@ -1,0 +1,32 @@
+module Main
+
+open BoyerMooreHorspool
+open Belongs
+open UpdateBc
+open GlobalData
+open ItemIndices
+open NewOrOld
+open FStar.Classical 
+open FStar.IO
+open FStar.Printf
+open FStar.List
+open FStar.List.Tot.Base
+
+//output verification
+let rec convert_english_letters_to_int (l:list english_letters)
+  : list int 
+  = match l with 
+    | [] -> []
+    | hd :: tl -> if hd = A then 
+                  0 :: convert_english_letters_to_int tl 
+                  else 1 :: convert_english_letters_to_int tl
+
+let main() =
+  let message =
+     sprintf "The result is %d." (boyer_moore_horspool text pattern 0 0)
+  in
+  print_string message
+
+#push-options "--warn_error -272"
+let _ = main()
+#pop-options
