NewOrOld.fst
@@ -1,0 +1,178 @@
+module NewOrOld
+
+open GlobalData
+open ItemIndices
+open FStar.Classical 
+open FStar.IO
+open FStar.Printf
+open FStar.List
+open FStar.List.Tot.Base
+
+let new_or_old (#a:eqtype) (c:a) (l:list a) : int
+  = if item_indices c l 0 <> []
+    then last (item_indices c l 0)
+    else -1
+
+let rec mem_last_list (#a:eqtype) (l:list a)
+  : Lemma (requires l <> [])
+          (ensures mem (last l) l = true)
+  = match l with 
+    | [el] -> ()
+    | hd :: tl -> mem_last_list tl
+
+let new_or_old_return_values (#a:eqtype) (l:list a) (item:a)
+  : Lemma (ensures new_or_old item l = -1 || (new_or_old item l >= 0 && new_or_old item l < length l))
+  = if item_indices item l 0 = []
+    then ()
+    else (
+      mem_last_list (item_indices item l 0);
+      item_indices_is_in_interval item l 0 (last (item_indices item l 0))
+    )
+
+let rec not_new_or_old_empty_list (#a:eqtype) (l:list a) (item:a)
+  : Lemma (ensures new_or_old item l = -1 ==> item_indices item l 0 = [])
+  = match l with
+    | [] -> ()
+    | hd :: tl -> not_new_or_old_empty_list tl item 
+
+let rec empty_list_length_zero (#a:eqtype) (l:list a) (item:a)
+  : Lemma (ensures item_indices item l 0 = [] ==> length (item_indices item l 0) = 0)
+  = match l with 
+    | [] -> ()
+    | hd :: tl -> empty_list_length_zero tl item
+
+let rec length_zero_count_zero (#a:eqtype) (l:list a) (item:a)
+  : Lemma (ensures length (item_indices item l 0) = 0 ==> count item l = 0)
+  = match l with
+    | [] -> ()
+    | hd :: tl -> length_zero_count_zero tl item;
+                  item_list_has_correct_length l 0
+
+let rec count_zero_mem_false (#a:eqtype) (l:list a) (item:a)
+  : Lemma (ensures count item l = 0 ==> mem item l = false)
+  = match l with
+    | [] -> ()
+    | hd :: tl -> count_zero_mem_false tl item
+                 
+let rec mem_false_not_item (#a:eqtype) (l:list a) (item:a) (i:nat{i < length l})
+  : Lemma (ensures mem item l = false ==> index l i <> item)
+  = match l with 
+    | [] -> ()
+    | hd :: tl -> match i with 
+                  | 0 -> ()
+                  | _ -> mem_false_not_item tl item (i - 1)
+
+let rec new_or_old_not_item_base (#a:eqtype) (l:list a) (item:a) (i:nat{i < length l})
+  : Lemma (ensures new_or_old item l = -1 ==> index l i <> item)
+  = match l with
+    | [] -> ()
+    | hd :: tl -> match i with 
+                  | 0 -> ()
+                  | _ -> new_or_old_not_item_base tl item (i - 1);
+                         not_new_or_old_empty_list l item;
+                         empty_list_length_zero l item;
+                         length_zero_count_zero l item;
+                         count_zero_mem_false l item;
+                         mem_false_not_item l item i
+
+let new_or_old_not_item (#a:eqtype) (l:list a) (item:a)
+  : Lemma (ensures forall (i:nat{i < length l}). new_or_old item l = -1 ==> index l i <> item)
+  = forall_intro (new_or_old_not_item_base l item)   
+
+let rec new_or_old_not_empty_list (#a:eqtype) (l:list a)
+  : Lemma (ensures forall (item:a). new_or_old item l <> -1 ==> item_indices item l 0 <> [])
+  = match l with
+    | [] -> ()
+    | hd :: tl -> new_or_old_not_empty_list tl
+
+let rec not_empty_list_mem_is_true_base (#a:eqtype) (l:list a) (item:a)
+  : Lemma (ensures item_indices item l 0 <> [] ==> mem (last (item_indices item l 0)) (item_indices item l 0) = true)
+  = match l with
+    | [] -> ()
+    | hd :: tl -> not_empty_list_mem_is_true_base tl item;
+                  if item_indices item l 0 <> []
+                  then mem_last_list (item_indices item l 0)
+                  else ()
+
+let not_empty_list_mem_is_true (#a:eqtype) (l:list a)
+  : Lemma (ensures forall (item:a). item_indices item l 0 <> [] ==> mem (last (item_indices item l 0)) (item_indices item l 0) = true)
+  = forall_intro (not_empty_list_mem_is_true_base l)
+ 
+let mem_index_is_item (#a:eqtype) (item:a) (l:list a)
+  : Lemma (requires item_indices item l 0 <> [] && last (item_indices item l 0) < length l)
+          (ensures mem (last (item_indices item l 0)) (item_indices item l 0) = true ==> index l (last (item_indices item l 0)) = item)
+  = mem_last_list (item_indices item l 0);
+    index_is_mem_is_item l
+
+let rec index_plus_one_base (#a:eqtype) (l:list a) (item:a) (el:a) (i:nat{i < length l})
+  : Lemma (ensures index l i = item ==> index (el :: l) (i + 1) = item)
+  = match l with
+    | [] -> ()
+    | hd :: tl -> match i with 
+                  | 0 -> ()
+                  | _ -> index_plus_one_base tl item hd (i - 1)
+
+let index_plus_one (#a:eqtype) (l:list a) (item:a) (el:a)
+  : Lemma (ensures forall (i:nat{i < length l}). index l i = item ==> index (el :: l) (i + 1) = item)
+  = forall_intro (index_plus_one_base l item el)
+
+let rec exists_tl_exists_tl_plus_hd (#a:eqtype) (l:list a) (item:a) (el:a)
+  : Lemma (ensures (exists (i:nat{i < length l}). index l i = item) ==> (exists (i:nat{i < length (el :: l)}). index (el :: l) i = item))
+  = match l with 
+    | [] -> ()
+    | hd :: tl -> if hd = item 
+                  then (
+                    assert(index l 0 = item);
+                    assert(index (el :: l) 1 = item)
+                  )
+                  else exists_tl_exists_tl_plus_hd tl item hd;
+                       index_plus_one l item el
+
+let rec mem_list_exists_index (#a:eqtype) (l:list a) (item:a)
+  : Lemma (ensures mem item l = true ==> (exists (i:nat{i < length l}). index l i = item))
+  = match l with 
+    | [] -> ()
+    | hd :: tl -> if hd = item 
+                  then assert(index l 0 = item)
+                  else (
+                    mem_list_exists_index tl item;
+                    exists_tl_exists_tl_plus_hd tl item hd
+                  )
+
+let index_in_list_is_less_than_last_base (#a:eqtype) (item:a) (l:list a{item_indices item l 0 <> []}) (x:nat)
+  : Lemma (ensures mem x (item_indices item l 0) = true ==> x <= last (item_indices item l 0))
+  = mem_list_exists_index (item_indices item l 0) x;
+    last_index_is_max item l;
+    last_is_length_l_minus_one (item_indices item l 0)
+
+let index_in_list_is_less_than_last (#a:eqtype) (item:a) (l:list a{item_indices item l 0 <> []})
+  : Lemma (ensures forall (i:nat). mem i (item_indices item l 0) = true ==> i <= last (item_indices item l 0))
+  = forall_intro (index_in_list_is_less_than_last_base item l)
+
+let index_greater_than_last_not_item (#a:eqtype) (item:a) (l:list a{item_indices item l 0 <> []}) (i:nat{i < length l})
+  : Lemma (ensures i > (last (item_indices item l 0)) ==> index l i <> item)
+  = index_is_not_mem_is_not_item_forall_i l item;
+    index_in_list_is_less_than_last item l
+
+let mem_index_is_item_last_indices_are_not_item_base (#a:eqtype) (item:a) (l:list a{item_indices item l 0 <> []}) (i:nat{i > (last (item_indices item l 0)) && i < length l})
+  : Lemma (ensures mem (last (item_indices item l 0)) (item_indices item l 0) = true ==> index l i <> item)
+  = index_greater_than_last_not_item item l i
+
+let mem_index_is_item_last_indices_are_not_item (#a:eqtype) (item:a) (l:list a{item_indices item l 0 <> []})
+  : Lemma (ensures mem (last (item_indices item l 0)) (item_indices item l 0) = true ==> (forall (i:nat{i > (last (item_indices item l 0)) && i < length l}). index l i <> item))
+  = forall_intro (index_greater_than_last_not_item item l)
+
+let mem_index_is_item_gives_correct_result (#a:eqtype) (l:list a) (item:a)
+  : Lemma (requires item_indices item l 0 <> [] && (last (item_indices item l 0)) < length l)
+          (ensures mem (last (item_indices item l 0)) (item_indices item l 0) = true ==> index l (last (item_indices item l 0)) = item /\ 
+          (forall (i:nat{i > (last (item_indices item l 0)) && i < length l}). index l i <> item))
+  = mem_index_is_item item l;
+    mem_index_is_item_last_indices_are_not_item item l
+
+let new_or_old_not_empty_list_correct_item (#a:eqtype) (l:list a) (item:a)
+  : Lemma (requires item_indices item l 0 <> [] && last (item_indices item l 0) < length l)
+          (ensures new_or_old item l <> -1 ==> index l (last (item_indices item l 0)) = item /\ 
+          (forall (i:nat{i > (last (item_indices item l 0)) && i < length l}). index l i <> item))
+  = new_or_old_not_empty_list l;
+    not_empty_list_mem_is_true l;
+    mem_index_is_item_gives_correct_result l item
