UpdateBc.fst
@@ -1,0 +1,124 @@
+module UpdateBc
+
+open GlobalData
+open ItemIndices
+open NewOrOld
+open FStar.Classical 
+open FStar.IO
+open FStar.Printf
+open FStar.List
+open FStar.List.Tot.Base
+
+let rec update_bc (a:list english_letters) (p:list english_letters) 
+  : list int
+  = match a with 
+    | [] -> []
+    | hd :: tl -> (new_or_old hd p) :: update_bc tl p
+
+let rec update_bc_length_is_initial_list_length (l:list english_letters) (p:list english_letters)
+  : Lemma (ensures length (update_bc l p) = length l)
+  = match l with 
+    | [] -> ()
+    | hd :: tl -> update_bc_length_is_initial_list_length tl p
+
+let rec update_bc_for_minusone_base (l:list english_letters) (p:list english_letters)
+                                    (i:nat{i < length l && i < length (update_bc l p)}) 
+                                    (j:nat{j < length p})
+  : Lemma (ensures 
+           (let l' = update_bc l p in
+            index l' i = -1 ==> index p j <> index l i))
+  = update_bc_length_is_initial_list_length l p;
+    match l with 
+    | [] -> ()
+    | fst :: tl -> match i with 
+                   | 0 -> assert(update_bc l p = (new_or_old fst p) :: update_bc tl p);
+                          assert(index (update_bc l p) i = new_or_old fst p);
+                          assert(fst = index l i);
+                          new_or_old_not_item_base p fst j;
+                          assert(new_or_old fst p = -1 ==> index p j <> fst)
+                   | _ -> update_bc_for_minusone_base tl p (i - 1) j
+
+let update_bc_for_minusone_forall_j (l:list english_letters) 
+                                    (p:list english_letters) 
+                                    (i:nat{i < length l && i < length (update_bc l p)})
+  : Lemma (ensures forall (j:nat{j < length p}).  
+           (let l' = update_bc l p in
+            index l' i = -1 ==> index p j <> index l i))
+  = forall_intro (update_bc_for_minusone_base l p i)
+
+let update_bc_for_minusone (l:list english_letters) (p:list english_letters)
+  : Lemma (ensures forall (i:nat{i < length l && i < length (update_bc l p)}). (forall (j:nat{j < length p}).  
+           (let l' = update_bc l p in
+            index l' i = -1 ==> index p j <> index l i)))
+  = forall_intro (update_bc_for_minusone_forall_j l p)
+
+let rec update_bc_for_nat_base (l:list english_letters)
+                               (p:list english_letters)
+                               (i:nat{i < length l && i < length (update_bc l p)}) 
+                               (j:nat{j < length p})
+  : Lemma (ensures 
+           (let l' = update_bc l p in
+            index l' i = j ==> index p j = index l i /\ (forall (i':nat{i' > j && i' < length p}). index p i' <> index l i)))
+  = update_bc_length_is_initial_list_length l p;
+    match l with 
+    | [] -> ()
+    | fst :: tl -> match i with 
+                   | 0 -> assert(update_bc l p = (new_or_old fst p) :: update_bc tl p);
+                          assert(index (update_bc l p) i = new_or_old fst p);
+                          assert(fst = index l i);
+                          if j = new_or_old fst p
+                          then (
+                            if item_indices (index l i) l 0 <> []
+                            then (
+                              item_indices_is_in_interval (index l i) l 0 (last (item_indices (index l i) l 0));
+                              new_or_old_not_empty_list_correct_item p fst
+                            )
+                            else ()
+                          )
+                          else ()
+                   | _ -> update_bc_for_nat_base tl p (i - 1) j
+
+let update_bc_for_nat_forall_j (l:list english_letters) 
+                               (p:list english_letters)
+                               (i:nat{i < length l && i < length (update_bc l p)})
+  : Lemma (ensures 
+           (let l' = update_bc l p in forall (j:nat{j < length p}).
+            index l' i = j ==> index p j = index l i /\ (forall (i':nat{i' > j && i' < length p}). index p i' <> index l i)))
+  = forall_intro (update_bc_for_nat_base l p i)
+
+let update_bc_for_nat (l:list english_letters) (p:list english_letters)
+  : Lemma (ensures 
+           (let l' = update_bc l p in forall (i:nat{i < length l && i < length (update_bc l p)}) (j:nat{j < length p}).
+            index l' i = j ==> index p j = index l i /\ 
+            (forall (i':nat{i' > j && i' < length p}). index p i' <> index l i)))
+  = forall_intro (update_bc_for_nat_forall_j l p)
+
+let rec update_bc_has_values_in_interval (l:list english_letters) (p:list english_letters) (i:nat{i < length (update_bc l p)})
+  : Lemma (ensures 
+           (let l' = update_bc l p in 
+            index l' i = -1 || (index l' i >= 0 && index l' i < length p)))
+  = match l with 
+    | [] -> ()
+    | fst :: tl -> if i = 0 
+                   then new_or_old_return_values p fst
+                   else update_bc_has_values_in_interval tl p  (i - 1)
+
+let final_bc : list int = update_bc alphabet pattern
+
+let update_bc_has_index_minusone_if_letter_is_not_in_pattern_for_alphabet ()
+  : Lemma (ensures forall (i:nat{i < length alphabet && i < length (update_bc alphabet pattern)}). (forall (j:nat{j < length pattern}).  
+           (let l' = update_bc alphabet pattern in
+            index l' i = -1 ==> index pattern j <> index alphabet i)))
+  = update_bc_for_minusone alphabet pattern
+
+let update_bc_has_correct_index_if_letter_is_in_pattern_for_alphabet ()
+  : Lemma (ensures 
+           (let l' = update_bc alphabet pattern in forall 
+            (i:nat{i < length alphabet && i < length (update_bc alphabet pattern)}) (j:nat{j < length pattern}).
+            index l' i = j ==> index pattern j = index alphabet i /\ 
+            (forall (i':nat{i' > j && i' < length pattern}). index pattern i' <> index alphabet i)))
+  = update_bc_for_nat alphabet pattern
+
+let final_bc_has_same_length_as_alphabet () 
+  : Lemma (ensures length final_bc = length alphabet)
+  = update_bc_length_is_initial_list_length alphabet pattern
